theories/Staging/NewShallow/Executor.v
@@ -42,9 +42,9 @@ From Equations Require Import
 From Katamaran Require Import
      Notations
      Prelude
+     Sep.Hoare
      Sep.Logic
-     Signature
-     Specification.
+     Signature.
 
 From stdpp Require base list option.
 
@@ -62,11 +62,11 @@ Module Type NewShallowExecOn
   (Import B : Base)
   (Import SIG : Signature B)
   (Import PROG : Program B)
-  (Import SPEC : Specification B SIG PROG).
+  (Import PLOG : ProgramLogic B SIG PROG).
 
   Import iris.proofmode.tactics.
 
-  Module CPureSpecM.
+  Module CPureSpec.
   Section WithProp.
 
     Context {L} {biA : BiAffine L} {PI : PredicateDef L}.
@@ -76,10 +76,10 @@ Module Type NewShallowExecOn
     (* The pure backwards predicate transformer monad. We use this monad in some
        of the definition of primitives that do no need access to the store and
        that can later be lifted to the proper monad. *)
-    Definition CPureSpecM (A : Type) : Type :=
+    Definition CPureSpec (A : Type) : Type :=
       (A -> L) -> L.
 
-    Definition Monotonic {A} : relation (CPureSpecM A) :=
+    Definition Monotonic {A} : relation (CPureSpec A) :=
       (A ::> (⊢)) ==> (⊢).
 
     #[export] Instance monotonic_transitive {A} : Transitive (@Monotonic A).
@@ -87,6 +87,18 @@ Module Type NewShallowExecOn
       intros f g h fg gh P Q PQ. transitivity (g Q).
       apply fg. assumption. apply gh. reflexivity.
     Qed.
+
+    (* For counting the different execution paths of the shallow executor we use
+     different aliases for False and True to distinguish between them. TRUE
+     and FALSE represent execution paths that are pruned, i.e. do not reach
+     the end of a function, and FINISH encodes the successful execution
+     case. *)
+    Definition FALSE : L := False.
+    Definition TRUE : L := True.
+    Definition FINISH : L := True.
+    #[global] Typeclasses Opaque TRUE.
+    #[global] Typeclasses Opaque FALSE.
+    #[global] Typeclasses Opaque FINISH.
 
     Local Ltac solve_wp :=
       repeat
@@ -125,36 +137,27 @@ Module Type NewShallowExecOn
          end).
 
     Section Basic.
-      Definition pure {A : Type} :
-        A -> CPureSpecM A :=
+      Definition run : CPureSpec unit → L :=
+        (* We use the FINISH alias of True for the purpose
+         of counting nodes in a shallowly-generated VC. *)
+        fun m => m (fun _ => FINISH).
+
+      Definition pure {A : Type} : A → CPureSpec A :=
         fun a POST => POST a.
       #[global] Arguments pure {A} a _ /.
 
-      Definition map {A B} :
-        (A -> B) -> CPureSpecM A -> CPureSpecM B :=
+      Definition map {A B} : (A → B) → CPureSpec A → CPureSpec B :=
         fun f m POST => m (Basics.compose POST f).
       #[global] Arguments map {A B} f m _ /.
 
       Definition bind {A B} :
-        CPureSpecM A -> (A -> CPureSpecM B) -> CPureSpecM B :=
+        CPureSpec A → (A → CPureSpec B) → CPureSpec B :=
         fun m f POST => m (fun a1 => f a1 POST).
       #[global] Arguments bind {A B} ma f _ /.
 
-      (* For counting the different execution paths of the shallow executor we use
-         different aliases for False and True to distinguish between them. TRUE
-         and FALSE represent execution paths that are pruned, i.e. do not reach
-         the end of a function, and FINISH encodes the successful execution
-         case. *)
-      Definition FALSE : L := False.
-      Definition TRUE : L := True.
-      Definition FINISH : L := True.
-      Global Typeclasses Opaque TRUE.
-      Global Typeclasses Opaque FALSE.
-      Global Typeclasses Opaque FINISH.
-
-      Definition error {A} : CPureSpecM A :=
+      Definition error {A} : CPureSpec A :=
         fun POST => FALSE.
-      Definition block {A} : CPureSpecM A :=
+      Definition block {A} : CPureSpec A :=
         fun POST => TRUE.
 
     End Basic.
@@ -165,12 +168,12 @@ Module Type NewShallowExecOn
 
     Section Nondeterminism.
 
-      Definition angelic (σ : Ty) : CPureSpecM (Val σ) :=
+      Definition angelic (σ : Ty) : CPureSpec (Val σ) :=
         fun POST => (∃ v : Val σ, POST v)%I.
       #[global] Arguments angelic σ _ /.
 
       Definition angelic_ctx {N : Set} :
-        forall Δ : NCtx N Ty, CPureSpecM (NamedEnv Val Δ) :=
+        forall Δ : NCtx N Ty, CPureSpec (NamedEnv Val Δ) :=
         fix rec Δ {struct Δ} :=
           match Δ with
           | [ctx]   => pure [env]
@@ -180,12 +183,12 @@ Module Type NewShallowExecOn
           end.
       #[global] Arguments angelic_ctx {N} Δ.
 
-      Definition demonic σ : CPureSpecM (Val σ) :=
+      Definition demonic σ : CPureSpec (Val σ) :=
         fun POST => (∀ v : Val σ, POST v)%I.
       #[global] Arguments demonic σ _ /.
 
       Definition demonic_ctx {N : Set} :
-        forall Δ : NCtx N Ty, CPureSpecM (NamedEnv Val Δ) :=
+        forall Δ : NCtx N Ty, CPureSpec (NamedEnv Val Δ) :=
         fix rec Δ {struct Δ} :=
           match Δ with
           | [ctx]   => pure [env]
@@ -196,49 +199,49 @@ Module Type NewShallowExecOn
       #[global] Arguments demonic_ctx {N} Δ.
 
       Definition angelic_binary {A} :
-        CPureSpecM A -> CPureSpecM A -> CPureSpecM A :=
+        CPureSpec A -> CPureSpec A -> CPureSpec A :=
         fun m1 m2 POST =>
           (m1 POST ∨ m2 POST)%I.
       Definition demonic_binary {A} :
-        CPureSpecM A -> CPureSpecM A -> CPureSpecM A :=
+        CPureSpec A -> CPureSpec A -> CPureSpec A :=
         fun m1 m2 POST =>
           (m1 POST ∧ m2 POST)%I.
 
       Definition angelic_list' {A} :
-        A -> list A -> CPureSpecM A :=
+        A -> list A -> CPureSpec A :=
         fix rec d xs :=
           match xs with
           | nil        => pure d
           | cons x xs  => angelic_binary (pure d) (rec x xs)
           end.
 
-      Definition angelic_list {A} (xs : list A) : CPureSpecM A :=
+      Definition angelic_list {A} (xs : list A) : CPureSpec A :=
         match xs with
         | nil       => error
         | cons x xs => angelic_list' x xs
         end.
 
       Definition demonic_list' {A} :
-        A -> list A -> CPureSpecM A :=
+        A -> list A -> CPureSpec A :=
         fix rec d xs :=
           match xs with
           | nil        => pure d
           | cons x xs  => demonic_binary (pure d) (rec x xs)
           end.
 
-      Definition demonic_list {A} (xs : list A) : CPureSpecM A :=
+      Definition demonic_list {A} (xs : list A) : CPureSpec A :=
         match xs with
         | nil       => block
         | cons x xs => demonic_list' x xs
         end.
 
       Definition angelic_finite F `{finite.Finite F} :
-        CPureSpecM F :=
+        CPureSpec F :=
         angelic_list (finite.enum F).
       #[global] Arguments angelic_finite F {_ _}.
 
       Definition demonic_finite F `{finite.Finite F} :
-        CPureSpecM F :=
+        CPureSpec F :=
         demonic_list (finite.enum F).
       #[global] Arguments demonic_finite F {_ _}.
 
@@ -304,16 +307,16 @@ Module Type NewShallowExecOn
 
     Section Guards.
 
-      Definition assume_formula (fml : Prop) : CPureSpecM unit :=
+      Definition assume_formula (fml : Prop) : CPureSpec unit :=
         fun POST => (⌜fml⌝ → POST tt)%I.
       #[global] Arguments assume_formula _ _ /.
-      Definition assert_formula (fml : Prop) : CPureSpecM unit :=
+      Definition assert_formula (fml : Prop) : CPureSpec unit :=
         fun POST => (⌜fml⌝ ∧ POST tt)%I.
       #[global] Arguments assert_formula _ _ /.
-      Definition produce_chunk (c : SCChunk) : CPureSpecM unit :=
+      Definition produce_chunk (c : SCChunk) : CPureSpec unit :=
         fun POST => (interpret_scchunk c -∗ POST tt)%I.
       #[global] Arguments produce_chunk c _ /.
-      Definition consume_chunk (c : SCChunk) : CPureSpecM unit :=
+      Definition consume_chunk (c : SCChunk) : CPureSpec unit :=
         fun POST => (interpret_scchunk c ∗ POST tt)%I.
       #[global] Arguments consume_chunk c _/.
 
@@ -322,13 +325,13 @@ Module Type NewShallowExecOn
          terms. We mirror the structure of the symbolic execution and also
          traverse (the statically known parts) of other data structures. *)
       Equations(noeqns) assert_eq_env [Δ : Ctx Ty]
-        (δ δ' : Env Val Δ) : CPureSpecM unit :=
+        (δ δ' : Env Val Δ) : CPureSpec unit :=
         assert_eq_env env.nil          env.nil            := pure tt;
         assert_eq_env (env.snoc δ _ t) (env.snoc δ' _ t') :=
           bind (assert_eq_env δ δ') (fun _ => assert_formula (t = t')).
 
       Equations(noeqns) assert_eq_nenv {N : Set} [Δ : NCtx N Ty]
-        (δ δ' : NamedEnv Val Δ) : CPureSpecM unit :=
+        (δ δ' : NamedEnv Val Δ) : CPureSpec unit :=
         assert_eq_nenv env.nil          env.nil            := pure tt;
         assert_eq_nenv (env.snoc δ _ t) (env.snoc δ' _ t') :=
           bind (assert_eq_nenv δ δ') (fun _ => assert_formula (t = t')).
@@ -381,8 +384,8 @@ Module Type NewShallowExecOn
     Section PatternMatching.
 
       Definition pattern_match {N : Set} {A σ} (v : Val σ) (pat : Pattern (N:=N) σ)
-        (k : forall (pc : PatternCase pat), NamedEnv Val (PatternCaseCtx pc) -> CPureSpecM A) :
-        CPureSpecM A :=
+        (k : forall (pc : PatternCase pat), NamedEnv Val (PatternCaseCtx pc) -> CPureSpec A) :
+        CPureSpec A :=
         fun POST => let (pc,δpc) := pattern_match_val pat v in k pc δpc POST.
       #[global] Arguments pattern_match {N A σ} v pat  _ /.
 
@@ -390,7 +393,7 @@ Module Type NewShallowExecOn
 
     Section ProduceConsume.
 
-      Fixpoint produce {Σ} (ι : Valuation Σ) (asn : Assertion Σ) : CPureSpecM unit :=
+      Fixpoint produce {Σ} (asn : Assertion Σ) (ι : Valuation Σ) : CPureSpec unit :=
         match asn with
         | asn.formula fml => assume_formula (instprop fml ι)
         | asn.chunk c     => produce_chunk (inst c ι)
@@ -399,18 +402,19 @@ Module Type NewShallowExecOn
             pattern_match
               (inst (T := fun Σ => Term Σ _) s ι)
               pat
-              (fun pc δpc => produce (ι ►► δpc) (rhs pc))
-        | asn.sep a1 a2   => _ <- produce ι a1 ;; produce ι a2
+              (fun pc δpc => produce (rhs pc) (ι ►► δpc))
+        | asn.sep a1 a2   => _ <- produce a1 ι ;; produce a2 ι
         | asn.or a1 a2 =>
-          demonic_binary (produce ι a1)
-                         (produce ι a2)
+            demonic_binary
+              (produce a1 ι)
+              (produce a2 ι)
         | asn.exist ς τ a =>
           v <- demonic τ ;;
-          produce (env.snoc ι (ς∷τ) v) a
+          produce a (env.snoc ι (ς∷τ) v)
         | asn.debug => pure tt
         end.
 
-      Fixpoint consume {Σ} (ι : Valuation Σ) (asn : Assertion Σ) : CPureSpecM unit :=
+      Fixpoint consume {Σ} (asn : Assertion Σ) (ι : Valuation Σ) : CPureSpec unit :=
         match asn with
         | asn.formula fml => assert_formula (instprop fml ι)
         | asn.chunk c     => consume_chunk (inst c ι)
@@ -419,19 +423,17 @@ Module Type NewShallowExecOn
             pattern_match
               (inst (T := fun Σ => Term Σ _) s ι)
               pat
-              (fun pc δpc => consume (ι ►► δpc) (rhs pc))
-        | asn.sep a1 a2   => _ <- consume ι a1;; consume ι a2
-        | asn.or a1 a2 =>
-          angelic_binary (consume ι a1)
-                         (consume ι a2)
+              (fun pc δpc => consume (rhs pc) (ι ►► δpc))
+        | asn.sep a1 a2   => _ <- consume a1 ι ;; consume a2 ι
+        | asn.or a1 a2 => angelic_binary (consume a1 ι) (consume a2 ι)
         | asn.exist ς τ a =>
           v <- angelic τ ;;
-          consume (env.snoc ι (ς∷τ) v) a
+          consume a (env.snoc ι (ς∷τ) v)
         | asn.debug => pure tt
         end.
 
       Lemma wp_produce {Σ} {ι : Valuation Σ} {asn : Assertion Σ} (POST : unit -> L) :
-        produce ι asn POST ⊣⊢ (asn.interpret asn ι -∗ POST tt).
+        produce asn ι POST ⊣⊢ (asn.interpret asn ι -∗ POST tt).
       Proof.
         revert POST. induction asn; cbn - [inst inst_term]; intros POST.
         - apply wp_assume_formula.
@@ -447,7 +449,7 @@ Module Type NewShallowExecOn
       Qed.
 
       Lemma wp_consume {Σ} {ι : Valuation Σ} {asn : Assertion Σ} (POST : unit -> L) :
-        consume ι asn POST ⊣⊢ asn.interpret asn ι ∗ POST tt.
+        consume asn ι POST ⊣⊢ asn.interpret asn ι ∗ POST tt.
       Proof.
         revert POST. induction asn; cbn - [inst inst_term]; intros POST.
         - apply wp_assert_formula.
@@ -467,19 +469,19 @@ Module Type NewShallowExecOn
     Section Calls.
 
       Definition call_contract {Δ τ} (ctr : SepContract Δ τ) (args : CStore Δ) :
-        CPureSpecM (Val τ) :=
+        CPureSpec (Val τ) :=
           match ctr with
           | MkSepContract _ _ Σe δ req result ens =>
             ι <- angelic_ctx Σe ;;
             assert_eq_nenv args (inst δ ι) ;;
-            consume ι req  ;;
+            consume req ι ;;
             v <- demonic τ ;;
-            produce (env.snoc ι (result∷τ) v) ens ;;
+            produce ens (env.snoc ι (result∷τ) v) ;;
             pure v
           end.
 
       Definition call_contract' {Δ τ} (ctr : SepContract Δ τ) (args : CStore Δ) :
-        CPureSpecM (Val τ) :=
+        CPureSpec (Val τ) :=
         fun POST =>
           match ctr with
           | MkSepContract _ _ Σe δ req result ens =>
@@ -487,16 +489,16 @@ Module Type NewShallowExecOn
               asn.interpret req ι ∗ (∀ v : Val τ, asn.interpret ens ι.[result∷τ ↦ v] -∗ POST v)
           end%I.
 
-      Definition call_lemma {Δ} (lem : Lemma Δ) (args : CStore Δ) : CPureSpecM unit :=
+      Definition call_lemma {Δ} (lem : Lemma Δ) (args : CStore Δ) : CPureSpec unit :=
           match lem with
           | MkLemma _ Σe δ req ens =>
             ι <- angelic_ctx Σe ;;
             assert_eq_nenv args (inst δ ι) ;;
-            consume ι req ;;
-            produce ι ens
+            consume req ι ;;
+            produce ens ι
           end.
 
-      Definition call_lemma' {Δ} (lem : Lemma Δ) (args : CStore Δ) : CPureSpecM (Val ty.unit) :=
+      Definition call_lemma' {Δ} (lem : Lemma Δ) (args : CStore Δ) : CPureSpec (Val ty.unit) :=
         fun POST =>
           match lem with
           | MkLemma _ Σe δ req ens =>
@@ -545,11 +547,28 @@ Module Type NewShallowExecOn
     End Calls.
 
   End WithProp.
-  End CPureSpecM.
-  Export CPureSpecM (CPureSpecM).
-  #[export] Hint Unfold CPureSpecM.Monotonic : typeclass_instances.
 
-  Module CHeapSpecM.
+  Module notations.
+
+    Infix "⊗" := demonic_binary (at level 40, left associativity) : mut_scope.
+    Infix "⊕" := angelic_binary (at level 50, left associativity) : mut_scope.
+
+    Notation "' x <- ma ;; mb" :=
+      (bind ma (fun x => mb))
+        (at level 80, x pattern, ma at next level, mb at level 200, right associativity,
+           format "' x  <-  ma  ;;  mb") : mut_scope.
+    Notation "x <- ma ;; mb" :=
+      (bind ma (fun x => mb))
+        (at level 80, ma at level 90, mb at level 200, right associativity) : mut_scope.
+      (* Notation "ma >>= f" := (bind ma f) (at level 50, left associativity) : mut_scope. *)
+
+  End notations.
+
+  End CPureSpec.
+  Export CPureSpec (CPureSpec).
+  #[export] Hint Unfold CPureSpec.Monotonic : typeclass_instances.
+
+  Module CStoreSpec.
   Section WithProp.
 
     Context {L} {biA : BiAffine L} {PI : PredicateDef L}.
@@ -562,9 +581,31 @@ Module Type NewShallowExecOn
     Bind Scope mut_scope with CHeapSpecM.
     Local Open Scope mut_scope.
 
+    (* The paper discusses the case that a function call is replaced by
+       interpreting the contract instead. However, this is not always
+       convenient. We therefore make contracts for functions optional and if a
+       function does not have a contract, we continue executing the body of
+       the called function. A parameter [inline_fuel] bounds the number of
+       allowed levels before failing execution. Therefore, we write the
+       executor in an open-recusion style and [Exec] is the closed type of
+       such an executor. *)
+    Definition ExecCall := forall Δ τ, 𝑭 Δ τ -> CStore Δ -> CPureSpec (L := L) (Val τ).
+    Definition ExecCallForeign := forall Δ τ, 𝑭𝑿 Δ τ -> CStore Δ -> CPureSpec (L := L) (Val τ).
+    Definition ExecLemma := forall Δ, 𝑳 Δ -> CStore Δ -> CPureSpec (L := L) unit.
+    Definition ExecFail := forall Γ τ (s : Val ty.string), CHeapSpecM Γ Γ (Val τ).
+    Definition Exec := forall Γ τ (s : Stm Γ τ), CHeapSpecM Γ Γ (Val τ).
+
+    Definition ExecRefine (e1 e2 : Exec) : Prop :=
+      forall Γ τ (s : Stm Γ τ) POST δ,
+        e1 _ _ s POST δ ⊢ e2 _ _ s POST δ.
+
     Section Basic.
 
-      Definition lift_purem {Γ A} (m : CPureSpecM A) : CHeapSpecM Γ Γ A :=
+      Definition evalStoreSpec {Γ1 Γ2 A} :
+        CHeapSpecM Γ1 Γ2 A -> CStore Γ1 -> CPureSpec A :=
+        fun m δ Φ => m (fun a1 _ => Φ a1) δ.
+
+      Definition lift_purem {Γ A} (m : CPureSpec A) : CHeapSpecM Γ Γ A :=
         fun POST δ => m (fun a => POST a δ).
       #[global] Arguments lift_purem {Γ A} m _ /.
 
@@ -603,25 +644,6 @@ Module Type NewShallowExecOn
     #[local] Notation "ma ;; mb" := (bind_right ma mb) : mut_scope.
     #[local] Infix "⊗" := demonic_binary (at level 40, left associativity) : mut_scope.
     #[local] Infix "⊕" := angelic_binary (at level 50, left associativity) : mut_scope.
-
-    (* Module CHeapSpecMNotations. *)
-
-    (*   Infix "⊗" := demonic_binary (at level 40, left associativity) : mut_scope. *)
-    (*   Infix "⊕" := angelic_binary (at level 50, left associativity) : mut_scope. *)
-
-    (*   Notation "' x <- ma ;; mb" := *)
-    (*     (bind ma (fun x => mb)) *)
-    (*       (at level 80, x pattern, ma at next level, mb at level 200, right associativity, *)
-    (*        format "' x  <-  ma  ;;  mb") : mut_scope. *)
-    (*   Notation "x <- ma ;; mb" := *)
-    (*     (bind ma (fun x => mb)) *)
-    (*       (at level 80, ma at level 90, mb at level 200, right associativity) : mut_scope. *)
-    (*   (* Notation "ma >>= f" := (bind ma f) (at level 50, left associativity) : mut_scope. *) *)
-    (*   Notation "ma ;; mb" := (bind_right ma mb) : mut_scope. *)
-
-    (* End CHeapSpecMNotations. *)
-    (* Import CHeapSpecMNotations. *)
-    (* Local Open Scope mut_scope. *)
 
     Section PatternMatching.
 
@@ -662,425 +684,468 @@ Module Type NewShallowExecOn
 
     End State.
 
-    Section Exec.
+    Section ExecAux.
 
-      (* The paper discusses the case that a function call is replaced by
-         interpreting the contract instead. However, this is not always
-         convenient. We therefore make contracts for functions optional and if a
-         function does not have a contract, we continue executing the body of
-         the called function. A parameter [inline_fuel] bounds the number of
-         allowed levels before failing execution. Therefore, we write the
-         executor in an open-recusion style and [Exec] is the closed type of
-         such an executor. *)
-      Definition Exec := forall Γ τ (s : Stm Γ τ), CHeapSpecM Γ Γ (Val τ).
-      Definition ExecCall := forall Δ τ, 𝑭 Δ τ -> CStore Δ -> CPureSpecM (L := L) (Val τ).
+      Context {SPEC : Specification}.
+      Variable exec_call_foreign : ExecCallForeign.
+      Variable exec_lemma : ExecLemma.
+      Variable exec_call : ExecCall.
+      Variable exec_fail : ExecFail.
 
-      Definition ExecRefine (e1 e2 : Exec) : Prop :=
-        forall Γ τ (s : Stm Γ τ) POST δ,
-          e1 _ _ s POST δ ⊢ e2 _ _ s POST δ.
-
-      Section ExecOpen.
-
-        (* The executor for "inlining" a call. *)
-        Variable exec : Exec.
-
-        Definition exec_call_inline : ExecCall :=
-          fun Δ τ f args POST =>
-            exec (FunDef f) (fun v _ => POST v) args.
-
-        Definition exec_call_with_contracts : ExecCall :=
-          fun Δ τ f args =>
-            match CEnv f with
-            | Some c => CPureSpecM.call_contract c args
-            | None   => exec_call_inline f args
-            end.
-
-        Variable exec_call : ExecCall.
-
-        (* The openly-recursive executor. *)
-        Definition exec_open : Exec :=
-          fun Γ τ s =>
-            match s with
-            | stm_val _ l => pure l
-            | stm_exp e => eval_exp e
-            | stm_let x σ s k =>
-              v <- exec s ;;
-              pushpop v (exec k)
-            | stm_block δ k =>
-              pushspops δ (exec k)
-            | stm_assign x e =>
-              v <- exec e ;;
-              _ <- assign x v ;;
-              pure v
-            | stm_call f es =>
-              args <- eval_exps es ;;
-              lift_purem (exec_call f args)
-            | stm_foreign f es =>
-              ts <- eval_exps es ;;
-              lift_purem (CPureSpecM.call_contract (CEnvEx f) ts)
-            | stm_lemmak l es k =>
-              ts <- eval_exps es ;;
-              _  <- lift_purem (CPureSpecM.call_lemma (LEnv l) ts) ;;
-              exec k
-            | stm_call_frame δ' s =>
-              δ <- get_local ;;
-              _ <- put_local δ' ;;
-              v <- exec s ;;
-              _ <- put_local δ ;;
-              pure v
-            | stm_seq e k => _ <- exec e ;; exec k
-            | stm_assertk e1 _ k =>
-              v <- eval_exp e1 ;;
-              _ <- lift_purem (CPureSpecM.assume_formula (v = true)) ;;
-              exec k
-            | stm_fail _ s =>
-              block
-            | stm_pattern_match s pat rhs =>
-              v <- exec s ;;
-              pattern_match v pat
-                (fun pc δpc => pushspops δpc (exec (rhs pc)))
-            | stm_read_register reg =>
-              v <- angelic τ ;;
-              let c := chunk_ptsreg reg v in
-              _ <- lift_purem (CPureSpecM.consume_chunk c) ;;
-              _ <- lift_purem (CPureSpecM.produce_chunk c) ;;
-              pure v
-            | stm_write_register reg e =>
-              v__old <- angelic τ ;;
-              _    <- lift_purem (CPureSpecM.consume_chunk (chunk_ptsreg reg v__old)) ;;
-              v__new <- eval_exp e ;;
-              _    <- lift_purem (CPureSpecM.produce_chunk (chunk_ptsreg reg v__new)) ;;
-              pure v__new
-            | stm_bind s k =>
-              v <- exec s ;;
-              exec (k v)
-            | stm_debugk k =>
-              exec k
-            end.
-
-      End ExecOpen.
-      #[global] Arguments exec_call_with_contracts exec [_ _] f args _ /.
-
-      Definition exec_error : Exec :=
-        fun _ _ _ => error.
-      Definition exec_def (rec : Exec) : Exec :=
-        exec_open rec (exec_call_inline rec).
-      Definition exec_aux (exec_call : ExecCall) : Exec :=
-        fix exec_aux Γ τ s := exec_open exec_aux exec_call s.
-
-      (* The constructed closed executor. *)
-      Fixpoint exec (inline_fuel : nat) : Exec :=
-        match inline_fuel with
-        | O   => exec_error
-        | S n => exec_aux (exec_call_with_contracts (exec n))
-        end.
-      #[global] Arguments exec _ [_ _] s _ _.
-
-    End Exec.
-
-    Section WithFuel.
-
-      Variable inline_fuel : nat.
-
-      Definition exec_contract {Δ τ} (c : SepContract Δ τ) (s : Stm Δ τ) :
-       Valuation (sep_contract_logic_variables c) -> CHeapSpecM Δ Δ unit :=
-        match c with
-        | MkSepContract _ _ _ _ req result ens =>
-          fun ι =>
-          _ <- lift_purem (CPureSpecM.produce ι req) ;;
-          v <- exec inline_fuel s ;;
-          lift_purem (CPureSpecM.consume (env.snoc ι (result∷τ) v) ens)
-        end%mut.
-
-      Definition vcgen {Δ τ} (c : SepContract Δ τ) (body : Stm Δ τ) : Prop :=
-        ForallNamed (fun ι : Valuation (sep_contract_logic_variables c) =>
-          let δΔ : CStore Δ := inst (sep_contract_localstore c) ι in
-          (* We use the FINISH alias of True for the purpose of counting
-             nodes in a shallowly-generated VC. *)
-          ⊢ exec_contract c body ι (fun _ _ => CPureSpecM.FINISH) δΔ).
-
-      Definition vcgen' {Δ τ} (c : SepContract Δ τ) (body : Stm Δ τ) : Prop :=
-        match c with
-        | MkSepContract _ _ Σ δ req result ens =>
-            forall ι : Valuation Σ,
-              asn.interpret req ι ⊢
-              exec inline_fuel body
-                (fun v _ => asn.interpret ens (env.snoc ι (result∷τ) v)) (inst δ ι)
-        end.
-
-    End WithFuel.
-
-    (* This section verifies the monotonicity of the calculated predicate
-       transformers. Which is a necessity for the main soundness theorems. *)
-    Section Monotonicity.
-
-      #[local] Open Scope signature.
-
-      Definition Monotonic {Γ1 Γ2 A} : relation (CHeapSpecM Γ1 Γ2 A) :=
-        (A ::> CStore Γ2 ::> (⊢)) ==> CStore Γ1 ::> (⊢).
-      Definition Monotonic' {Γ1 Γ2 A} : relation (CHeapSpecM Γ1 Γ2 A) :=
-        (A -> CStore Γ2 -> L) ::> CStore Γ1 ::> (⊢).
-
-      Definition MonotonicExec : relation Exec :=
-        ∀ Γ τ, Stm Γ τ ::> Monotonic.
-      Definition MonotonicExec' : relation Exec :=
-        ∀ Γ τ, Stm Γ τ ::> Monotonic'.
-      Definition MonotonicCall : relation ExecCall :=
-        ∀ Δ σ, 𝑭 Δ σ ::> CStore Δ ::> CPureSpecM.Monotonic.
-
-      #[export] Instance monotonic_transitive {Γ1 Γ2 A} :
-        Transitive (@Monotonic Γ1 Γ2 A).
-      Proof.
-        intros f g h fg gh P Q PQ δ. transitivity (g Q δ).
-        apply fg. assumption. apply gh. reflexivity.
-      Qed.
-
-      #[export] Instance monotonicexec_transitive :
-        Transitive MonotonicExec.
-      Proof.
-        intros f g h fg gh Γ τ s.
-        transitivity (g Γ τ s); [apply fg|apply gh].
-      Qed.
-
-      Ltac solve_monotonic :=
-        repeat
-          lazymatch goal with
-          | |- ?x           ⊢ ?x => reflexivity
-          | |- Basics.flip (⊢) ?x ?y => change_no_check (y ⊢ x)
-          | |- bi_impl _ _    ⊢ _  => apply bi.impl_mono'; [easy|]
-          | |- bi_sep _ _     ⊢ _  => apply bi.sep_mono'
-          | |- bi_wand _ _    ⊢ _  => apply bi.wand_mono'
-          | |- bi_exist _     ⊢ _  => apply bi.exist_mono'; intros ?
-          | H : (_ ::> CStore _ ::> (⊢)) ?P ?Q |- ?P ?x ?δ ⊢ ?Q ?x ?δ =>
-              apply H
-          | H : Monotonic ?m1 ?m2 |- ?m1 _ ?δ ⊢ ?m2 _ ?δ =>
-              apply H; intros ? ?
-          | H: MonotonicExec ?ex1 ?ex2 |- ?ex1 _ _ ?s _ _ ⊢ ?ex2 _ _ ?s _ _ =>
-              apply H; intros ? ?
-          | H: MonotonicCall ?ec1 ?ec2 |- ?ec1 _ _ ?f _ _ ⊢ ?ec2 _ _ ?f _ _ =>
-              apply H; intros ?
-          | H: Proper MonotonicCall ?ec |- ?ec _ _ ?f _ _ ⊢ ?ec _ _ ?f _ _ =>
-              apply H; intros ?
-          (* | H: forall _, Monotonic (?f _) (?g _) |- ?f _ _ ?δ ⊢ ?g _ _ ?δ => *)
-          (*     apply H; intros ? ? *)
-          | H: forall _, Monotonic (?f _ _ _) (?g _ _ _) |- ?f _ _ _ _ _ ⊢ ?g _ _ _ _ _ =>
-              apply H; intros ? ?
-          | |- CPureSpecM.call_contract _ _ _ ⊢ _ =>
-              apply CPureSpecM.monotonic_call_contract; intros ?
-          | |- CPureSpecM.call_lemma _ _ _ ⊢ _ =>
-              apply CPureSpecM.monotonic_call_lemma; intros ?
-          | |- (match ?x with _ => _ end) ⊢ _ => destruct x
-          | |- Proper _ _ => unfold Proper
-          | |- Monotonic _ _ => intros ?P ?Q ?PQ ?δ; cbn
-          | |- respectful _ _ _ _ => intros ? ? ?
-          | H: (_ ::> Monotonic) ?f ?g |- ?f _ _ _ ⊢ ?g _ _ _ =>
-              apply H; intros ? ?
+      (* The openly-recursive executor. *)
+      Definition exec_aux : Exec :=
+        fix exec {Γ τ} (s : Stm Γ τ) : CHeapSpecM Γ Γ (Val τ) :=
+          match s with
+          | stm_val _ l => pure l
+          | stm_exp e => eval_exp e
+          | stm_let x σ s k =>
+            v <- exec s ;;
+            pushpop v (exec k)
+          | stm_block δ k =>
+            pushspops δ (exec k)
+          | stm_assign x e =>
+            v <- exec e ;;
+            _ <- assign x v ;;
+            pure v
+          | stm_call f es =>
+            args <- eval_exps es ;;
+            lift_purem (exec_call f args)
+          | stm_foreign f es =>
+            ts <- eval_exps es ;;
+            lift_purem (exec_call_foreign f ts)
+          | stm_lemmak l es k =>
+            ts <- eval_exps es ;;
+            _  <- lift_purem (exec_lemma l ts) ;;
+            exec k
+          | stm_call_frame δ' s =>
+            δ <- get_local ;;
+            _ <- put_local δ' ;;
+            v <- exec s ;;
+            _ <- put_local δ ;;
+            pure v
+          | stm_seq e k => _ <- exec e ;; exec k
+          | stm_assertk e1 _ k =>
+            v <- eval_exp e1 ;;
+            _ <- lift_purem (CPureSpec.assert_formula
+                               (if fail_rule_pre then True else v <> false)) ;;
+            _ <- lift_purem (CPureSpec.assume_formula (v = true)) ;;
+            exec k
+          | stm_fail _ s =>
+            exec_fail _ s
+          | stm_pattern_match s pat rhs =>
+            v <- exec s ;;
+            pattern_match v pat
+              (fun pc δpc => pushspops δpc (exec (rhs pc)))
+          | stm_read_register reg =>
+            v <- angelic τ ;;
+            let c := chunk_ptsreg reg v in
+            _ <- lift_purem (CPureSpec.consume_chunk c) ;;
+            _ <- lift_purem (CPureSpec.produce_chunk c) ;;
+            pure v
+          | stm_write_register reg e =>
+            v__old <- angelic τ ;;
+            _    <- lift_purem (CPureSpec.consume_chunk (chunk_ptsreg reg v__old)) ;;
+            v__new <- eval_exp e ;;
+            _    <- lift_purem (CPureSpec.produce_chunk (chunk_ptsreg reg v__new)) ;;
+            pure v__new
+          | stm_bind s k =>
+            v <- exec s ;;
+            exec (k v)
+          | stm_debugk k =>
+            exec k
           end.
 
-      Instance exec_call_inline_monotonic :
-        Proper (MonotonicExec ==> MonotonicCall) (exec_call_inline).
-      Proof. intros ex1 ex2 ex_mon Δ σ f args P Q PQ. now apply ex_mon. Qed.
-
-      Instance exec_call_with_contracts_monotonic :
-        Proper (MonotonicExec ==> MonotonicCall) (exec_call_with_contracts).
-      Proof.
-        intros ex1 ex2 ex_mon Δ σ f args.
-        unfold exec_call_with_contracts. destruct CEnv.
-        - apply CPureSpecM.monotonic_call_contract.
-        - now apply exec_call_inline_monotonic.
-      Qed.
-
-      Instance exec_open_monotonic :
-        Proper (MonotonicExec ==> MonotonicCall ==> MonotonicExec) exec_open.
-      Proof.
-        intros ex1 ex2 ex_mon ec1 ec2 ec_mon Γ τ s P Q PQ δΓ.
-        destruct s; cbn; solve_monotonic.
-      Qed.
-
-      Instance exec_def_monotonic :
-        Proper (MonotonicExec ==> MonotonicExec) exec_def.
-      Proof.
-        intros ex1 ex2 ex_mon. unfold exec_def.
-        now apply exec_open_monotonic, exec_call_inline_monotonic.
-      Qed.
-
-      Instance exec_aux_monotonic :
-        Proper (MonotonicCall ==> MonotonicExec) (exec_aux).
-      Proof.
-        intros ec1 ec2 ec_mon Γ τ s.
-        induction s; intros P Q PQ ?; cbn; solve_monotonic.
-      Qed.
-
-      Lemma fold_exec_aux (ex : Exec) (ec : ExecCall)
-        (IHc : Proper MonotonicCall ec)
-        (IHx : MonotonicExec (exec_open ex ec) ex) :
-        MonotonicExec (exec_aux ec) ex.
-      Proof.
-        intros Γ τ s; induction s; cbn [exec_aux];
-          match goal with
-          | |- Monotonic (exec_open _ _ ?s) (ex _ _ ?s) =>
-              transitivity (exec_open ex ec s);
-              [cbn [exec_open]|apply IHx]
-          end;
-          solve_monotonic.
-      Qed.
-
-      Lemma exec_error_initial (ex : Exec) :
-        MonotonicExec exec_error ex.
-      Proof. intros ? ? ? ? ? ? ?. apply bi.False_elim. Qed.
-
-      Lemma exec_monotonic n : Proper MonotonicExec (exec n).
-      Proof.
-        induction n; cbn.
-        - apply exec_error_initial.
-        - now apply exec_aux_monotonic, exec_call_with_contracts_monotonic.
-      Qed.
-
-      Record Model (ex : Exec) : Prop := {
-          rule_syntactic :
-            MonotonicExec'
-              (exec_def ex)
-              ex;
-
-          rule_contract :
-            MonotonicCall
-              (exec_call_with_contracts exec_error)
-              (exec_call_inline ex);
-
-          ex_monotonic :> Proper MonotonicExec ex;
-        }.
-
-    End Monotonicity.
-
-    Lemma vcgen_equiv {Δ τ} n (c : SepContract Δ τ) (body : Stm Δ τ) :
-      vcgen n c body <-> vcgen' n c body.
-    Proof.
-      destruct c as [Σ δ req result ens]; cbn. unfold CPureSpecM.FINISH.
-      rewrite env.Forall_forall. apply all_iff_morphism; intros ι.
-      rewrite CPureSpecM.wp_produce entails_wand_iff.
-      apply bi.bi_emp_valid_proper. apply bi.wand_proper; [easy|].
-      apply bi.entails_anti_sym; apply exec_monotonic; intros v δ';
-        now rewrite CPureSpecM.wp_consume ?bi.sep_True ?bi.True_sep.
-    Qed.
+    End ExecAux.
+    #[global] Arguments exec_aux {SPEC} _ _ _ _ [Γ τ] !s.
 
   End WithProp.
-  End CHeapSpecM.
-  Export CHeapSpecM (CHeapSpecM).
+  Module notations.
 
+    Infix "⊗" := demonic_binary (at level 40, left associativity) : mut_scope.
+    Infix "⊕" := angelic_binary (at level 50, left associativity) : mut_scope.
+
+      Notation "' x <- ma ;; mb" :=
+        (bind ma (fun x => mb))
+          (at level 80, x pattern, ma at next level, mb at level 200, right associativity,
+           format "' x  <-  ma  ;;  mb") : mut_scope.
+      Notation "x <- ma ;; mb" :=
+        (bind ma (fun x => mb))
+          (at level 80, ma at level 90, mb at level 200, right associativity) : mut_scope.
+      (* Notation "ma >>= f" := (bind ma f) (at level 50, left associativity) : mut_scope. *)
+      Notation "ma ;; mb" := (bind_right ma mb) : mut_scope.
+
+  End notations.
+  End CStoreSpec.
+
+  Section WithExec.
+
+    Import CPureSpec.notations CStoreSpec.
+
+    Context {L} {biA : BiAffine L} {PI : PredicateDef L}.
+    Context (exec : Exec (L := L)).
+
+    Definition exec_contract {Δ τ} (c : SepContract Δ τ) (s : Stm Δ τ) : CPureSpec unit :=
+      match c with
+      | MkSepContract _ _ lvars pats req result ens =>
+          lenv <- CPureSpec.demonic_ctx lvars ;;
+          _    <- CPureSpec.produce req lenv ;;
+          v    <- CStoreSpec.evalStoreSpec (exec s) (inst pats lenv) ;;
+          CPureSpec.consume ens (env.snoc lenv (result∷τ) v)
+      end%mut.
+
+    (* Lemma mon_exec_contract {Δ τ} (c : SepContract Δ τ) (s : Stm Δ τ) : *)
+    (*   CPureSpec.Monotonic CPureSpec.Monotonic (exec_contract c s). *)
+    (* Proof. destruct c. typeclasses eauto. Qed. *)
+
+  End WithExec.
+
+  Section WithSpec.
+
+    Import CPureSpec.notations CStoreSpec.
+
+    Context {L} {biA : BiAffine L} {PI : PredicateDef L}.
+    Context (exec : Exec (L := L)).
+
+    Definition exec_call_error_no_fuel : ExecCall (L := L) :=
+      fun Δ τ f args => CPureSpec.error.
+
+    Definition cexec_call_foreign {SPEC : Specification} : ExecCallForeign :=
+      fun Δ τ f args =>
+        CPureSpec.call_contract (CEnvEx f) args.
+
+    Definition debug_lemma [Δ] (f : 𝑳 Δ) (args : CStore Δ) : CPureSpec (L := L) unit :=
+      CPureSpec.pure tt.
+
+    Open Scope mut_scope.
+
+    Definition cexec_lemma {SPEC : Specification} : ExecLemma (L := L) :=
+      fun Δ l args =>
+        _ <- debug_lemma l args ;;
+        CPureSpec.call_lemma (LEnv l) args.
+
+    Definition debug_call [Δ τ] (f : 𝑭 Δ τ) (args : CStore Δ) : CPureSpec (L := L) unit :=
+      CPureSpec.pure tt.
+
+    Definition cexec_fail {SPEC : Specification} : ExecFail (L := L) :=
+      fun Γ τ s => if fail_rule_pre then CStoreSpec.block else CStoreSpec.error.
+
+    (* If a function does not have a contract, we continue executing the body of
+       the called function. A parameter [inline_fuel] bounds the number of
+       allowed levels before failing execution. *)
+    Fixpoint cexec_call {SPEC : Specification} (inline_fuel : nat) : ExecCall :=
+      fun Δ τ f args =>
+        _ <- debug_call f args ;;
+        (* Let's first see if we have a contract defined for function [f]
+           and then if we have enough fuel for inlining. *)
+        match CEnv f , inline_fuel with
+        | Some c , _ =>
+            (* YES: Execute the call by interpreting the contract. *)
+            CPureSpec.call_contract c args
+        | None   , 0 =>
+            (* Out of fuel *)
+            exec_call_error_no_fuel f args
+        | None   , S n =>
+            CStoreSpec.evalStoreSpec
+              (CStoreSpec.exec_aux cexec_call_foreign cexec_lemma
+                 (cexec_call n) cexec_fail (FunDef f))
+              args
+        end.
+
+    Definition cexec {SPEC : Specification} (inline_fuel : nat) : Exec :=
+      @CStoreSpec.exec_aux _ _ SPEC cexec_call_foreign cexec_lemma
+        (cexec_call inline_fuel) cexec_fail.
+    #[global] Arguments cexec {_} _ [_ _] s _ _ : simpl never.
+
+    Definition vcgen {SPEC : Specification} (inline_fuel : nat) {Δ τ} (c : SepContract Δ τ) (body : Stm Δ τ) : L :=
+      CPureSpec.run (exec_contract (cexec inline_fuel) c body).
+
+    Import (hints) CStoreSpec.
+
+    (* Lemma mon_exec_call_error_no_fuel : MonotonicExecCall exec_call_error_no_fuel. *)
+    (* Proof. typeclasses eauto. Qed. *)
+
+    (* Lemma mon_cexec_call_foreign {SPEC : Specification} : *)
+    (*   MonotonicExecCallForeign cexec_call_foreign. *)
+    (* Proof. typeclasses eauto. Qed. *)
+
+    (* Lemma mon_cexec_lemma {SPEC : Specification} : *)
+    (*   MonotonicExecLemma cexec_lemma. *)
+    (* Proof. typeclasses eauto. Qed. *)
+
+    (* Lemma mon_cexec_fail {SPEC : Specification} : MonotonicExecFail cexec_fail. *)
+    (* Proof. unfold cexec_fail; destruct fail_rule_pre; typeclasses eauto. Qed. *)
+
+    (* #[export] Instance mon_cexec_call {SPEC : Specification} (fuel : nat) : *)
+    (*   MonotonicExecCall (cexec_call fuel). *)
+    (* Proof. *)
+    (*   induction fuel; intros; cbn; destruct CEnv; *)
+    (*     unfold cexec_fail; destruct fail_rule_pre; *)
+    (*     typeclasses eauto. *)
+    (* Qed. *)
+
+    (* Lemma mon_cexec {SPEC : Specification} (fuel : nat) : *)
+    (*   MonotonicExec (cexec fuel). *)
+    (* Proof. unfold cexec, cexec_fail; destruct fail_rule_pre; typeclasses eauto. Qed. *)
+
+    (* (* This section verifies the monotonicity of the calculated predicate *)
+    (*    transformers. Which is a necessity for the main soundness theorems. *) *)
+    (* Section Monotonicity. *)
+
+    (*   #[local] Open Scope signature. *)
+
+    (*   Definition Monotonic {Γ1 Γ2 A} : relation (CHeapSpecM (L := L) Γ1 Γ2 A) := *)
+    (*     (A ::> CStore Γ2 ::> (⊢)) ==> CStore Γ1 ::> (⊢). *)
+    (*   Definition Monotonic' {Γ1 Γ2 A} : relation (CHeapSpecM (L := L) Γ1 Γ2 A) := *)
+    (*     (A -> CStore Γ2 -> L) ::> CStore Γ1 ::> (⊢). *)
+
+    (*   Definition MonotonicExec : relation Exec := *)
+    (*     ∀ Γ τ, Stm Γ τ ::> Monotonic. *)
+    (*   Definition MonotonicExec' : relation Exec := *)
+    (*     ∀ Γ τ, Stm Γ τ ::> Monotonic'. *)
+    (*   Definition MonotonicCall : relation (ExecCall (L := L)) := *)
+    (*     ∀ Δ σ, 𝑭 Δ σ ::> CStore Δ ::> CPureSpec.Monotonic. *)
+
+    (*   #[export] Instance monotonic_transitive {Γ1 Γ2 A} : *)
+    (*     Transitive (@Monotonic Γ1 Γ2 A). *)
+    (*   Proof. *)
+    (*     intros f g h fg gh P Q PQ δ. transitivity (g Q δ). *)
+    (*     apply fg. assumption. apply gh. reflexivity. *)
+    (*   Qed. *)
+
+    (*   #[export] Instance monotonicexec_transitive : *)
+    (*     Transitive MonotonicExec. *)
+    (*   Proof. *)
+    (*     intros f g h fg gh Γ τ s. *)
+    (*     transitivity (g Γ τ s); [apply fg|apply gh]. *)
+    (*   Qed. *)
+
+    (*   Ltac solve_monotonic := *)
+    (*     repeat *)
+    (*       lazymatch goal with *)
+    (*       | |- ?x           ⊢ ?x => reflexivity *)
+    (*       | |- Basics.flip (⊢) ?x ?y => change_no_check (y ⊢ x) *)
+    (*       | |- bi_impl _ _    ⊢ _  => apply bi.impl_mono'; [easy|] *)
+    (*       | |- bi_sep _ _     ⊢ _  => apply bi.sep_mono' *)
+    (*       | |- bi_wand _ _    ⊢ _  => apply bi.wand_mono' *)
+    (*       | |- bi_and ?P _    ⊢ bi_and ?P _ => apply bi.and_mono' *)
+    (*       | |- bi_exist _     ⊢ _  => apply bi.exist_mono'; intros ? *)
+    (*       | H : (_ ::> CStore _ ::> (⊢)) ?P ?Q |- ?P ?x ?δ ⊢ ?Q ?x ?δ => *)
+    (*           apply H *)
+    (*       | H : Monotonic ?m1 ?m2 |- ?m1 _ ?δ ⊢ ?m2 _ ?δ => *)
+    (*           apply H; intros ? ? *)
+    (*       | H: MonotonicExec ?ex1 ?ex2 |- ?ex1 _ _ ?s _ _ ⊢ ?ex2 _ _ ?s _ _ => *)
+    (*           apply H; intros ? ? *)
+    (*       | H: MonotonicCall ?ec1 ?ec2 |- ?ec1 _ _ ?f _ _ ⊢ ?ec2 _ _ ?f _ _ => *)
+    (*           apply H; intros ? *)
+    (*       | H: Proper MonotonicCall ?ec |- ?ec _ _ ?f _ _ ⊢ ?ec _ _ ?f _ _ => *)
+    (*           apply H; intros ? *)
+    (*       (* | H: forall _, Monotonic (?f _) (?g _) |- ?f _ _ ?δ ⊢ ?g _ _ ?δ => *) *)
+    (*       (*     apply H; intros ? ? *) *)
+    (*       | H: forall _, Monotonic (?f _ _ _) (?g _ _ _) |- ?f _ _ _ _ _ ⊢ ?g _ _ _ _ _ => *)
+    (*           apply H; intros ? ? *)
+    (*       | |- CPureSpec.call_contract _ _ _ ⊢ _ => *)
+    (*           apply CPureSpec.monotonic_call_contract; intros ? *)
+    (*       | |- CPureSpec.call_lemma _ _ _ ⊢ _ => *)
+    (*           apply CPureSpec.monotonic_call_lemma; intros ? *)
+    (*       | |- (match ?x with _ => _ end) ⊢ _ => destruct x *)
+    (*       | |- Proper _ _ => unfold Proper *)
+    (*       | |- Monotonic _ _ => intros ?P ?Q ?PQ ?δ; cbn *)
+    (*       | |- respectful _ _ _ _ => intros ? ? ? *)
+    (*       | H: (_ ::> Monotonic) ?f ?g |- ?f _ _ _ ⊢ ?g _ _ _ => *)
+    (*           apply H; intros ? ? *)
+    (*       end. *)
+
+    (*   (* Instance exec_call_inline_monotonic : *) *)
+    (*   (*   Proper (MonotonicExec ==> MonotonicCall) (exec_call_inline). *) *)
+    (*   (* Proof. intros ex1 ex2 ex_mon Δ σ f args P Q PQ. now apply ex_mon. Qed. *) *)
+
+    (*   (* Instance exec_call_with_contracts_monotonic {SPEC : Specification} : *) *)
+    (*   (*   Proper (MonotonicExec ==> MonotonicCall) (exec_call_with_contracts). *) *)
+    (*   (* Proof. *) *)
+    (*   (*   intros ex1 ex2 ex_mon Δ σ f args. *) *)
+    (*   (*   unfold exec_call_with_contracts. destruct CEnv. *) *)
+    (*   (*   - apply CPureSpec.monotonic_call_contract. *) *)
+    (*   (*   - now apply exec_call_inline_monotonic. *) *)
+    (*   (* Qed. *) *)
+
+    (*   (* Instance exec_open_monotonic {SPEC : Specification} : *) *)
+    (*   (*   Proper (MonotonicExec ==> MonotonicCall ==> MonotonicExec) exec_open. *) *)
+    (*   (* Proof. *) *)
+    (*   (*   intros ex1 ex2 ex_mon ec1 ec2 ec_mon Γ τ s P Q PQ δΓ. *) *)
+    (*   (*   destruct s; cbn; solve_monotonic. *) *)
+    (*   (* Qed. *) *)
+
+    (*   (* Instance exec_def_monotonic {SPEC : Specification} : *) *)
+    (*   (*   Proper (MonotonicExec ==> MonotonicExec) exec_def. *) *)
+    (*   (* Proof. *) *)
+    (*   (*   intros ex1 ex2 ex_mon. unfold exec_def. *) *)
+    (*   (*   now apply exec_open_monotonic, exec_call_inline_monotonic. *) *)
+    (*   (* Qed. *) *)
+
+    (*   (* Instance exec_aux_monotonic {SPEC : Specification} : *) *)
+    (*   (*   Proper (MonotonicCall ==> MonotonicExec) (exec_aux). *) *)
+    (*   (* Proof. *) *)
+    (*   (*   intros ec1 ec2 ec_mon Γ τ s. *) *)
+    (*   (*   induction s; intros P Q PQ ?; cbn; solve_monotonic. *) *)
+    (*   (* Qed. *) *)
+
+    (*   (* Lemma fold_exec_aux {SPEC : Specification} (ex : Exec) (ec : ExecCall) *) *)
+    (*   (*   (IHc : Proper MonotonicCall ec) *) *)
+    (*   (*   (IHx : MonotonicExec (exec_open ex ec) ex) : *) *)
+    (*   (*   MonotonicExec (exec_aux ec) ex. *) *)
+    (*   (* Proof. *) *)
+    (*   (*   intros Γ τ s; induction s; cbn [exec_aux]; *) *)
+    (*   (*     match goal with *) *)
+    (*   (*     | |- Monotonic (exec_open _ _ ?s) (ex _ _ ?s) => *) *)
+    (*   (*         transitivity (exec_open ex ec s); *) *)
+    (*   (*         [cbn [exec_open]|apply IHx] *) *)
+    (*   (*     end; *) *)
+    (*   (*     solve_monotonic. *) *)
+    (*   (* Qed. *) *)
+
+    (*   (* Lemma exec_error_initial (ex : Exec) : *) *)
+    (*   (*   MonotonicExec exec_error ex. *) *)
+    (*   (* Proof. intros ? ? ? ? ? ? ?. apply bi.False_elim. Qed. *) *)
+
+    (*   (* Lemma exec_monotonic {SPEC : Specification} n : *) *)
+    (*   (*   Proper MonotonicExec (exec n). *) *)
+    (*   (* Proof. *) *)
+    (*   (*   induction n; cbn. *) *)
+    (*   (*   - apply exec_error_initial. *) *)
+    (*   (*   - now apply exec_aux_monotonic, exec_call_with_contracts_monotonic. *) *)
+    (*   (* Qed. *) *)
+
+    (*   (* Record Model {SPEC : Specification} (ex : Exec) : Prop := { *) *)
+    (*   (*     rule_syntactic : *) *)
+    (*   (*       MonotonicExec' *) *)
+    (*   (*         (exec_def ex) *) *)
+    (*   (*         ex; *) *)
+
+    (*   (*     rule_contract : *) *)
+    (*   (*       MonotonicCall *) *)
+    (*   (*         (exec_call_with_contracts exec_error) *) *)
+    (*   (*         (exec_call_inline ex); *) *)
+
+    (*   (*     ex_monotonic :> Proper MonotonicExec ex; *) *)
+    (*   (*   }. *) *)
+
+    (* End Monotonicity. *)
+
+  End WithSpec.
 
   Module Shallow.
 
     Section Soundness.
-      Context {L} {biA : BiAffine L} {PI : PredicateDef L}.
+      Context {L} {biA : BiAffine L} {PI : PredicateDef L} {SPEC : Specification}.
 
       Definition ValidContract {Δ τ} (c : SepContract Δ τ) (body : Stm Δ τ) : Prop :=
         (* Use inline_fuel = 1 by default. *)
-        CHeapSpecM.vcgen (L := L) 1 c body.
+        ⊢ vcgen (L := L) 1 c body.
 
       Definition ValidContractCEnv : Prop :=
         forall (Δ : PCtx) (τ : Ty) (f : 𝑭 Δ τ) (c : SepContract Δ τ),
           CEnv f = Some c ->
           ValidContract c (FunDef f).
 
-      Import CHeapSpecM.
+      (* Import CHeapSpecM. *)
 
-      Lemma rule_syntactic' (ec : ExecCall) (ec_mon : Proper MonotonicCall ec)
-        (ex : Exec) (ex_mdl : Model ex) :
-        MonotonicCall ec (exec_call_inline ex) ->
-        MonotonicExec (exec_aux ec) ex.
-      Proof.
-        intros. apply fold_exec_aux; [assumption|].
-        transitivity (exec_open ex (exec_call_inline ex)).
-        apply exec_open_monotonic.
-        apply ex_monotonic; auto.
-        assumption.
-        intros Γ τ s P Q PQ δ.
-        transitivity (ex _ _ s P δ).
-        apply (rule_syntactic ex_mdl).
-        apply ex_monotonic; auto.
-      Qed.
+      (* Lemma rule_syntactic' (ec : ExecCall) (ec_mon : Proper MonotonicCall ec) *)
+      (*   (ex : Exec) (ex_mdl : Model ex) : *)
+      (*   MonotonicCall ec (exec_call_inline ex) -> *)
+      (*   MonotonicExec (exec_aux ec) ex. *)
+      (* Proof. *)
+      (*   intros. apply fold_exec_aux; [assumption|]. *)
+      (*   transitivity (exec_open ex (exec_call_inline ex)). *)
+      (*   apply exec_open_monotonic. *)
+      (*   apply ex_monotonic; auto. *)
+      (*   assumption. *)
+      (*   intros Γ τ s P Q PQ δ. *)
+      (*   transitivity (ex _ _ s P δ). *)
+      (*   apply (rule_syntactic ex_mdl). *)
+      (*   apply ex_monotonic; auto. *)
+      (* Qed. *)
 
-      Definition ValidContractSem (ex : Exec) {Δ σ} (body : Stm Δ σ) (contract : SepContract Δ σ) : L :=
-        match contract with
-        | MkSepContract _ _ ctxΣ θΔ req res ens =>
-            ∀ (ι : Valuation ctxΣ),
-              asn.interpret req ι -∗
-               ex _ _ body (fun v _ => asn.interpret ens ι.[res∷σ ↦ v]) (inst θΔ ι)
-        end.
+      (* Definition ValidContractSem (ex : Exec) {Δ σ} (body : Stm Δ σ) (contract : SepContract Δ σ) : L := *)
+      (*   match contract with *)
+      (*   | MkSepContract _ _ ctxΣ θΔ req res ens => *)
+      (*       ∀ (ι : Valuation ctxΣ), *)
+      (*         asn.interpret req ι -∗ *)
+      (*          ex _ _ body (fun v _ => asn.interpret ens ι.[res∷σ ↦ v]) (inst θΔ ι) *)
+      (*   end. *)
 
-      Definition ValidContractEnvSem (ex : Exec) : L :=
-        ∀ Δ σ (f : 𝑭 Δ σ),
-          match CEnv f with
-          | Some c => ValidContractSem ex (FunDef f) c
-          | None   => True
-          end%I.
+      (* Definition ValidContractEnvSem (ex : Exec) : L := *)
+      (*   ∀ Δ σ (f : 𝑭 Δ σ), *)
+      (*     match CEnv f with *)
+      (*     | Some c => ValidContractSem ex (FunDef f) c *)
+      (*     | None   => True *)
+      (*     end%I. *)
 
-      Lemma validcontractsem_monotonic :
-        Proper
-          (MonotonicExec ==> ∀ Γ τ, Stm Γ τ ::> SepContract Γ τ ::> (⊢))
-          ValidContractSem.
-      Proof.
-        intros ex1 ex2 ex_mon Γ τ s [Σe δΔ req res ens]; cbn.
-        apply bi.forall_mono'; intros ι.
-        apply bi.wand_mono'; [easy|].
-        now apply ex_mon.
-      Qed.
+      (* Lemma validcontractsem_monotonic : *)
+      (*   Proper *)
+      (*     (MonotonicExec ==> ∀ Γ τ, Stm Γ τ ::> SepContract Γ τ ::> (⊢)) *)
+      (*     ValidContractSem. *)
+      (* Proof. *)
+      (*   intros ex1 ex2 ex_mon Γ τ s [Σe δΔ req res ens]; cbn. *)
+      (*   apply bi.forall_mono'; intros ι. *)
+      (*   apply bi.wand_mono'; [easy|]. *)
+      (*   now apply ex_mon. *)
+      (* Qed. *)
 
-      Instance validcontractenvsem_monotonic :
-        Proper (MonotonicExec ==> (⊢)) ValidContractEnvSem.
-      Proof.
-        intros ex1 ex2 ex_mon.
-        unfold ValidContractEnvSem.
-        apply bi.forall_mono'; intros Δ.
-        apply bi.forall_mono'; intros σ.
-        apply bi.forall_mono'; intros f.
-        destruct CEnv; [|easy].
-        now apply validcontractsem_monotonic.
-      Qed.
+      (* Instance validcontractenvsem_monotonic : *)
+      (*   Proper (MonotonicExec ==> (⊢)) ValidContractEnvSem. *)
+      (* Proof. *)
+      (*   intros ex1 ex2 ex_mon. *)
+      (*   unfold ValidContractEnvSem. *)
+      (*   apply bi.forall_mono'; intros Δ. *)
+      (*   apply bi.forall_mono'; intros σ. *)
+      (*   apply bi.forall_mono'; intros f. *)
+      (*   destruct CEnv; [|easy]. *)
+      (*   now apply validcontractsem_monotonic. *)
+      (* Qed. *)
 
-      Definition sound_shallow (vcenv : ValidContractCEnv) :
-        ⊢ ValidContractEnvSem (exec 1).
-      Proof.
-        iIntros (Δ σ f).
-        specialize (vcenv Δ σ f).
-        destruct (CEnv f) as [ctr|]; [|auto].
-        specialize (vcenv _ eq_refl).
-        unfold ValidContract in vcenv.
-        rewrite vcgen_equiv in vcenv.
-        destruct ctr as [Σe δΔ req res ens].
-        iIntros (ι) "Hreq".
-        specialize (vcenv ι).
-        now iApply vcenv.
-      Qed.
+      (* Definition sound_shallow (vcenv : ValidContractCEnv) : *)
+      (*   ⊢ ValidContractEnvSem (exec 1). *)
+      (* Proof. *)
+      (*   iIntros (Δ σ f). *)
+      (*   specialize (vcenv Δ σ f). *)
+      (*   destruct (CEnv f) as [ctr|]; [|auto]. *)
+      (*   specialize (vcenv _ eq_refl). *)
+      (*   unfold ValidContract in vcenv. *)
+      (*   rewrite vcgen_equiv in vcenv. *)
+      (*   destruct ctr as [Σe δΔ req res ens]. *)
+      (*   iIntros (ι) "Hreq". *)
+      (*   specialize (vcenv ι). *)
+      (*   now iApply vcenv. *)
+      (* Qed. *)
 
-      Lemma soundness (ex : Exec) (exmdl : Model ex) :
-        ValidContractCEnv -> ⊢ ValidContractEnvSem ex.
-      Proof.
-        unfold ValidContractCEnv.
-        intros vcenv.
-        apply bi.forall_intro. intros Δ.
-        apply bi.forall_intro. intros σ.
-        apply bi.forall_intro. intros f.
-        specialize (vcenv Δ σ f).
-        destruct (CEnv f) as [ctr|]; [|auto].
-        specialize (vcenv ctr eq_refl).
-        destruct ctr as [ctxΣ θΔ req res ens]; cbn in *.
-        apply bi.forall_intro. intros ι.
-        rewrite env.Forall_forall in vcenv.
-        change (emp ⊢ ?P) with (⊢ P).
-        specialize (vcenv ι). revert vcenv.
-        apply bi.bi_emp_valid_mono.
-        rewrite CPureSpecM.wp_produce.
-        apply bi.wand_mono'; [easy|].
-        apply rule_syntactic'; auto.
-        apply exec_call_with_contracts_monotonic.
-        apply exec_error_initial.
-        apply rule_contract; auto.
-        intros ? ?.
-        rewrite CPureSpecM.wp_consume.
-        unfold CPureSpecM.FINISH.
-        now rewrite bi.sep_True.
-      Qed.
+      (* Lemma soundness (ex : Exec) (exmdl : Model ex) : *)
+      (*   ValidContractCEnv -> ⊢ ValidContractEnvSem ex. *)
+      (* Proof. *)
+      (*   unfold ValidContractCEnv. *)
+      (*   intros vcenv. *)
+      (*   apply bi.forall_intro. intros Δ. *)
+      (*   apply bi.forall_intro. intros σ. *)
+      (*   apply bi.forall_intro. intros f. *)
+      (*   specialize (vcenv Δ σ f). *)
+      (*   destruct (CEnv f) as [ctr|]; [|auto]. *)
+      (*   specialize (vcenv ctr eq_refl). *)
+      (*   destruct ctr as [ctxΣ θΔ req res ens]; cbn in *. *)
+      (*   apply bi.forall_intro. intros ι. *)
+      (*   rewrite env.Forall_forall in vcenv. *)
+      (*   change (emp ⊢ ?P) with (⊢ P). *)
+      (*   specialize (vcenv ι). revert vcenv. *)
+      (*   apply bi.bi_emp_valid_mono. *)
+      (*   rewrite CPureSpec.wp_produce. *)
+      (*   apply bi.wand_mono'; [easy|]. *)
+      (*   apply rule_syntactic'; auto. *)
+      (*   apply exec_call_with_contracts_monotonic. *)
+      (*   apply exec_error_initial. *)
+      (*   apply rule_contract; auto. *)
+      (*   intros ? ?. *)
+      (*   rewrite CPureSpec.wp_consume. *)
+      (*   unfold CPureSpec.FINISH. *)
+      (*   now rewrite bi.sep_True. *)
+      (* Qed. *)
 
     End Soundness.
 
@@ -1110,9 +1175,9 @@ Module Type NewShallowExecOn
          number of different kinds of execution paths. *)
       Ltac reifyProp P :=
         match eval simpl in P with
-        | forall (x : ?T), CPureSpecM.TRUE => pspruned
-        | forall (x : ?T), CPureSpecM.FALSE => pspruned
-        | forall (x : ?T), CPureSpecM.FINISH => psfinish
+        | forall (x : ?T), CPureSpec.TRUE => pspruned
+        | forall (x : ?T), CPureSpec.FALSE => pspruned
+        | forall (x : ?T), CPureSpec.FINISH => psfinish
         | forall (x : ?T), True => psother
         | forall (x : ?T), False => psother
         | forall (x : ?T), @?P1 x /\ @?P2 x =>
@@ -1148,11 +1213,11 @@ Module Type NewShallowExecOn
 
         (* We make these instances global so that users can simply use the
            calc tactic qualified without importing the rest of this module. *)
-        #[global] Instance stats_true {L : bi} : ShallowStats CPureSpecM.TRUE :=
+        #[global] Instance stats_true {L : bi} : ShallowStats CPureSpec.TRUE :=
           {| branches := 1; pruned := 1 |}.
-        #[global] Instance stats_false : ShallowStats CPureSpecM.FALSE :=
+        #[global] Instance stats_false : ShallowStats CPureSpec.FALSE :=
           {| branches := 1; pruned := 1 |}.
-        #[global] Instance stats_finish : ShallowStats CPureSpecM.FINISH :=
+        #[global] Instance stats_finish : ShallowStats CPureSpec.FINISH :=
           {| branches := 1; pruned := 0 |}.
         (* We do not count regular True and False towards the statistics
            because they do not (should not) represent leaves of the shallow
@@ -1188,7 +1253,7 @@ Module Type NewShallowExecOn
       End WithSepLogic.
 
       Ltac calc fnc :=
-        let P := eval compute - [CPureSpecM.FALSE CPureSpecM.TRUE CPureSpecM.FINISH
+        let P := eval compute - [CPureSpec.FALSE CPureSpec.TRUE CPureSpec.FINISH
                                  negb Z.mul Z.opp Z.compare Z.add Z.geb Z.eqb
                                  Z.leb Z.gtb Z.ltb Z.le Z.lt Z.gt Z.ge Z.of_nat
                                  List.app List.length rev rev_append
@@ -1209,8 +1274,8 @@ Module MakeNewShallowExecutor
   (Import B    : Base)
   (Import SIG  : Signature B)
   (Import PROG : Program B)
-  (Import SPEC : Specification B SIG PROG).
+  (Import PLOG : ProgramLogic B SIG PROG).
 
-  Include NewShallowExecOn B SIG PROG SPEC.
+  Include NewShallowExecOn B SIG PROG PLOG.
 
 End MakeNewShallowExecutor.
