theories/Staging/NewShallow/Monads.v
@@ -1,0 +1,1035 @@
+(******************************************************************************)
+(* Copyright (c) 2020 Dominique Devriese, Sander Huyghebaert, Steven Keuchel  *)
+(* All rights reserved.                                                       *)
+(*                                                                            *)
+(* Redistribution and use in source and binary forms, with or without         *)
+(* modification, are permitted provided that the following conditions are     *)
+(* met:                                                                       *)
+(*                                                                            *)
+(* 1. Redistributions of source code must retain the above copyright notice,  *)
+(*    this list of conditions and the following disclaimer.                   *)
+(*                                                                            *)
+(* 2. Redistributions in binary form must reproduce the above copyright       *)
+(*    notice, this list of conditions and the following disclaimer in the     *)
+(*    documentation and/or other materials provided with the distribution.    *)
+(*                                                                            *)
+(* THIS SOFTWARE IS PROVIDED BY THE COPYRIGHT HOLDERS AND CONTRIBUTORS        *)
+(* "AS IS" AND ANY EXPRESS OR IMPLIED WARRANTIES, INCLUDING, BUT NOT LIMITED  *)
+(* TO, THE IMPLIED WARRANTIES OF MERCHANTABILITY AND FITNESS FOR A PARTICULAR *)
+(* PURPOSE ARE DISCLAIMED. IN NO EVENT SHALL THE COPYRIGHT HOLDER OR          *)
+(* CONTRIBUTORS BE LIABLE FOR ANY DIRECT, INDIRECT, INCIDENTAL, SPECIAL,      *)
+(* EXEMPLARY, OR CONSEQUENTIAL DAMAGES (INCLUDING, BUT NOT LIMITED TO,        *)
+(* PROCUREMENT OF SUBSTITUTE GOODS OR SERVICES; LOSS OF USE, DATA, OR         *)
+(* PROFITS; OR BUSINESS INTERRUPTION) HOWEVER CAUSED AND ON ANY THEORY OF     *)
+(* LIABILITY, WHETHER IN CONTRACT, STRICT LIABILITY, OR TORT (INCLUDING       *)
+(* NEGLIGENCE OR OTHERWISE) ARISING IN ANY WAY OUT OF THE USE OF THIS         *)
+(* SOFTWARE, EVEN IF ADVISED OF THE POSSIBILITY OF SUCH DAMAGE.               *)
+(******************************************************************************)
+
+From Coq Require Import
+  Classes.Morphisms
+  Classes.Morphisms_Prop
+  NArith.BinNat
+  Program.Basics
+  Relations.Relation_Definitions
+  ZArith.BinInt.
+From Equations Require Import
+  Equations.
+From Katamaran Require Import
+  Prelude
+  Base
+  Syntax.Assertions
+  Syntax.Chunks
+  Syntax.Predicates
+  Symbolic.Propositions
+  Symbolic.Worlds.
+
+Import SignatureNotations ctx.notations env.notations.
+
+#[local] Set Implicit Arguments.
+
+Module Type NewShallowMonadsOn (Import B : Base) (Import P : PredicateKit B)
+  (Import W : WorldsMixin B P) (Import SP : SymPropOn B P W)
+  (Import AS : AssertionsOn B P W).
+
+  Import iris.proofmode.tactics.
+
+  (* For counting the different execution paths of the shallow executor we use
+     different aliases for False and True to distinguish between them. TRUE
+     and FALSE represent execution paths that are pruned, i.e. do not reach
+     the end of a function, and FINISH encodes the successful execution
+     case. *)
+  Definition FALSE {L : bi} : L := False.
+  Definition TRUE {L : bi} : L := True.
+  Definition FINISH {L : bi} : L := True.
+  #[global] Typeclasses Opaque TRUE.
+  #[global] Typeclasses Opaque FALSE.
+  #[global] Typeclasses Opaque FINISH.
+
+  Module CPureSpec.
+
+    Section WithProp.
+
+      Context {L} {biA : BiAffine L} {PI : PredicateDef L}.
+      Bind Scope bi_scope with L.
+      Open Scope bi_scope.
+
+      (* The pure backwards predicate transformer monad. We use this monad in some
+         of the definition of primitives that do no need access to the store or heap
+         and that can later be lifted to the proper monad. *)
+      Definition CPureSpec (A : Type) : Type :=
+        (A → L) → L.
+
+      Definition run : CPureSpec unit -> L :=
+        (* We use the FINISH alias of True for the purpose
+           of counting nodes in a shallowly-generated VC. *)
+        fun m => m (fun _ => FINISH).
+
+      Definition pure {A : Type} : A -> CPureSpec A :=
+        fun a Φ => Φ a.
+      #[global] Arguments pure {A} a Φ /.
+
+      Definition bind {A B} :
+        CPureSpec A -> (A -> CPureSpec B) -> CPureSpec B :=
+        fun m f Φ => m (fun a1 => f a1 Φ).
+      #[global] Arguments bind {A B} m f _ /.
+      #[local] Notation "' x <- ma ;; mb" :=
+          (bind ma (fun x => mb))
+            (at level 80, x pattern, ma at next level, mb at level 200, right associativity,
+               format "' x  <-  ma  ;;  mb").
+      #[local] Notation "x <- ma ;; mb" :=
+        (bind ma (fun x => mb))
+          (at level 80, ma at level 90, mb at level 200, right associativity).
+      #[local] Notation "ma ;; mb" := (bind ma (fun _ => mb)).
+
+      Definition block {A} : CPureSpec A :=
+        fun Φ => TRUE.
+      Definition debug {A} : CPureSpec A -> CPureSpec A :=
+        fun m => m.
+      Definition error {A} : CPureSpec A :=
+        fun Φ => FALSE.
+
+      Definition assert_pathcondition : Prop -> CPureSpec unit :=
+        fun C Φ => ⌜C⌝ ∧ Φ tt.
+      Print assert_pathcondition.
+      Definition assume_pathcondition : Prop -> CPureSpec unit :=
+        fun C Φ => ⌜C⌝ → Φ tt.
+
+      Definition assert_formula : Prop -> CPureSpec unit :=
+        fun fml => assert_pathcondition fml.
+      Definition assume_formula : Prop -> CPureSpec unit :=
+        fun fml => assume_pathcondition fml.
+
+      Definition angelic_binary {A} :
+        CPureSpec A -> CPureSpec A -> CPureSpec A :=
+        fun m1 m2 Φ => m1 Φ ∨ m2 Φ.
+      Definition demonic_binary {A} :
+        CPureSpec A -> CPureSpec A -> CPureSpec A :=
+        fun m1 m2 Φ => m1 Φ ∧ m2 Φ.
+
+      Definition angelic (σ : Ty) : CPureSpec (Val σ) :=
+        fun Φ => ∃ (v : Val σ), Φ v.
+      Definition demonic (σ : Ty) : CPureSpec (Val σ) :=
+        fun Φ => ∀ (v : Val σ), Φ v.
+
+      (* Module Import notations. *)
+      (*   Notation "' x <- ma ;; mb" := *)
+      (*     (bind ma (fun x => mb)) *)
+      (*       (at level 80, x pattern, ma at next level, mb at level 200, right associativity, *)
+      (*          format "' x  <-  ma  ;;  mb"). *)
+      (*   Notation "x <- ma ;; mb" := *)
+      (*     (bind ma (fun x => mb)) *)
+      (*       (at level 80, ma at level 90, mb at level 200, right associativity). *)
+      (*   Notation "ma ;; mb" := (bind ma (fun _ => mb)). *)
+      (* End notations. *)
+
+      Definition angelic_ctx {N : Set} :
+        forall Δ : NCtx N Ty, CPureSpec (NamedEnv Val Δ) :=
+        fix rec Δ {struct Δ} :=
+          match Δ with
+          | [ctx]   => pure [env]
+          | Δ ▻ x∷σ => vs <- rec Δ;;
+                       v  <- angelic σ;;
+                       pure (vs ► (x∷σ ↦ v))
+          end.
+      #[global] Arguments angelic_ctx {N} Δ.
+
+      Definition demonic_ctx {N : Set} :
+        forall Δ : NCtx N Ty, CPureSpec (NamedEnv Val Δ) :=
+        fix rec Δ {struct Δ} :=
+          match Δ with
+          | []      => pure env.nil
+          | Δ ▻ x∷σ => vs <- rec Δ;;
+                       v  <- demonic σ;;
+                       pure (vs ► (x∷σ ↦ v))
+          end%ctx.
+      #[global] Arguments demonic_ctx {N} Δ.
+
+      Definition angelic_list' {A} :
+        A -> list A -> CPureSpec A :=
+        fix rec d xs :=
+          match xs with
+          | nil        => pure d
+          | cons x xs  => angelic_binary (pure d) (rec x xs)
+          end.
+
+      Definition angelic_list {A} (xs : list A) : CPureSpec A :=
+        match xs with
+        | nil => error
+        | cons x xs => angelic_list' x xs
+        end.
+
+      Definition demonic_list' {A} :
+        A -> list A -> CPureSpec A :=
+        fix rec d xs :=
+          match xs with
+          | nil        => pure d
+          | cons x xs  => demonic_binary (pure d) (rec x xs)
+          end.
+
+      Definition demonic_list {A} (xs : list A) : CPureSpec A :=
+        match xs with
+        | nil => block
+        | cons x xs => demonic_list' x xs
+        end.
+
+      Definition angelic_finite F `{finite.Finite F} : CPureSpec F :=
+        angelic_list (finite.enum F).
+      #[global] Arguments angelic_finite F {_ _}.
+
+      Definition demonic_finite F `{finite.Finite F} : CPureSpec F :=
+        demonic_list (finite.enum F).
+      #[global] Arguments demonic_finite F {_ _}.
+
+      Section PatternMatching.
+
+        Context {N : Set}.
+
+        Definition angelic_pattern_match {σ} (pat : Pattern (N:=N) σ)
+          (v : Val σ) : CPureSpec (MatchResult pat) :=
+          pc <- angelic_finite (PatternCase pat);;
+          vs <- angelic_ctx (PatternCaseCtx pc) ;;
+          _  <- assert_formula (pattern_match_val_reverse pat pc vs = v);;
+          pure (existT pc vs).
+        #[global] Arguments angelic_pattern_match {σ} pat v.
+
+        Definition demonic_pattern_match {σ} (pat : Pattern (N:=N) σ)
+          (v : Val σ) : CPureSpec (MatchResult pat) :=
+          pc <- demonic_finite (PatternCase pat);;
+          vs <- demonic_ctx (PatternCaseCtx pc) ;;
+          _  <- assume_formula (pattern_match_val_reverse pat pc vs = v);;
+          pure (existT pc vs).
+        #[global] Arguments demonic_pattern_match {σ} pat v.
+
+        Definition new_pattern_match {σ} (pat : Pattern (N:=N) σ)
+          (v : Val σ) : CPureSpec (MatchResult pat) :=
+          pure (pattern_match_val pat v).
+        #[global] Arguments new_pattern_match {σ} !pat v /.
+
+      End PatternMatching.
+
+      (* The paper uses asserted equalities between multiple types, but the
+         symbolic executor can in fact only assert equalities between symbolic
+         terms. We mirror the structure of the symbolic execution and also
+         traverse (the statically known parts) of other data structures. *)
+      Equations(noeqns) assert_eq_env [Δ : Ctx Ty]
+        (δ δ' : Env Val Δ) : CPureSpec unit :=
+        assert_eq_env env.nil          env.nil            := pure tt;
+        assert_eq_env (env.snoc δ _ t) (env.snoc δ' _ t') :=
+          bind (assert_eq_env δ δ') (fun _ => assert_formula (t = t')).
+
+      Equations(noeqns) assert_eq_nenv {N : Set} [Δ : NCtx N Ty]
+        (δ δ' : NamedEnv Val Δ) : CPureSpec unit :=
+        assert_eq_nenv env.nil          env.nil            := pure tt;
+        assert_eq_nenv (env.snoc δ _ t) (env.snoc δ' _ t') :=
+          bind (assert_eq_nenv δ δ') (fun _ => assert_formula (t = t')).
+
+      Equations(noeqns) assume_eq_env [Δ : Ctx Ty]
+        (δ δ' : Env Val Δ) : CPureSpec unit :=
+        assume_eq_env env.nil          env.nil            := pure tt;
+        assume_eq_env (env.snoc δ _ t) (env.snoc δ' _ t') :=
+          bind (assume_eq_env δ δ') (fun _ => assume_formula (t = t')).
+
+      Equations(noeqns) assume_eq_nenv {N : Set} [Δ : NCtx N Ty]
+        (δ δ' : NamedEnv Val Δ) : CPureSpec unit :=
+        assume_eq_nenv env.nil          env.nil            := pure tt;
+        assume_eq_nenv (env.snoc δ _ t) (env.snoc δ' _ t') :=
+          bind (assume_eq_nenv δ δ') (fun _ => assume_formula (t = t')).
+
+      Fixpoint assert_eq_chunk (c1 c2 : SCChunk) : CPureSpec unit :=
+        match c1 , c2 with
+        | chunk_user p1 vs1 , chunk_user p2 vs2 =>
+            match eq_dec p1 p2 with
+            | left e => assert_eq_env (eq_rect p1 (fun p => Env Val (𝑯_Ty p)) vs1 p2 e) vs2
+            | right _ => error
+            end
+        | chunk_ptsreg r1 v1 , chunk_ptsreg r2 v2 =>
+            match eq_dec_het r1 r2 with
+            | left e => assert_formula (eq_rect _ Val v1 _ (f_equal projT1 e) = v2)
+            | right _ => error
+            end
+        | chunk_conj c11 c12 , chunk_conj c21 c22 =>
+            assert_eq_chunk c11 c21 ;; assert_eq_chunk c12 c22
+        | chunk_wand c11 c12 , chunk_wand c21 c22 =>
+            assert_eq_chunk c11 c21 ;; assert_eq_chunk c12 c22
+        | _ , _ => error
+        end.
+
+      Definition replay_aux :
+        forall {Σ} (s : 𝕊 Σ) (ι : Valuation Σ), CPureSpec unit :=
+        fix replay {Σ} s ι :=
+          match s with
+          | SymProp.angelic_binary o1 o2 =>
+              angelic_binary (replay o1 ι) (replay o2 ι)
+          | SymProp.demonic_binary o1 o2 =>
+              demonic_binary (replay o1 ι) (replay o2 ι)
+          | SymProp.block =>
+              block
+          | SymProp.error msg =>
+              error
+          | SymProp.assertk fml msg k =>
+              assert_formula (instprop fml ι) ;;
+              replay k ι
+          | SymProp.assumek fml k =>
+              assume_formula (instprop fml ι) ;;
+              replay k ι
+          | SymProp.angelicv b k =>
+              v <- angelic _ ;;
+              replay k (env.snoc ι b v)
+          | SymProp.demonicv b k =>
+              v <- demonic _ ;;
+              replay k (env.snoc ι b v )
+          | @SymProp.assert_vareq _ x σ xIn t msg k =>
+              let ι' := env.remove (x ∷ σ) ι xIn in
+              let x' := ι.[? x∷σ] in
+              let t' := inst t ι' in
+              assert_formula (t' = x') ;;
+              replay k ι'
+          | @SymProp.assume_vareq _ x σ xIn t k =>
+              let ι' := env.remove (x ∷ σ) ι xIn in
+              let x' := ι.[? x∷σ] in
+              let t' := inst t ι' in
+              assume_formula (t' = x') ;;
+              replay k ι'
+          | SymProp.pattern_match s pat rhs =>
+              error
+          | SymProp.pattern_match_var x pat rhs =>
+              error
+          | SymProp.debug b k =>
+              debug (replay k ι)
+          end.
+
+      Definition replay [Σ] (P : 𝕊 Σ) (ι : Valuation Σ) : L :=
+        run (replay_aux P ι).
+
+      Definition produce_chunk (c : SCChunk) (h : SCHeap) : CPureSpec SCHeap :=
+        pure (cons c h).
+
+      Definition consume_chunk (c : SCChunk) (h : SCHeap) : CPureSpec SCHeap :=
+        '(c', h') <- angelic_list (heap_extractions h) ;;
+        assert_eq_chunk c c' ;;
+        pure h'.
+
+      Definition read_register {τ} (reg : 𝑹𝑬𝑮 τ) (h0 : SCHeap) : CPureSpec (Val τ * SCHeap) :=
+        v  <- angelic _ ;;
+        h1 <- consume_chunk (chunk_ptsreg reg v) h0 ;;
+        h2 <- produce_chunk (chunk_ptsreg reg v) h1 ;;
+        pure (v , h2).
+
+      Definition write_register {τ} (reg : 𝑹𝑬𝑮 τ) (vnew : Val τ) (h0 : SCHeap) :
+        CPureSpec (Val τ * SCHeap) :=
+        vold <- angelic _ ;;
+        h1   <- consume_chunk (chunk_ptsreg reg vold) h0 ;;
+        h2   <- produce_chunk (chunk_ptsreg reg vnew) h1 ;;
+        pure (vnew, h2).
+
+    Local Ltac solve_wp :=
+      repeat
+        (try progress subst;
+         lazymatch goal with
+         (* These first rules do not change the provability if the goal, i.e.
+            these steps are always complete. *)
+         | x : NamedEnv Val [ctx] |- _ => destruct (env.view x)
+         | x: NamedEnv Val (_ ▻ _) |- _ => destruct (env.view x)
+         | |- _ ⊣⊢ _ => apply bi.entails_anti_sym
+         | |- False ⊢ _ => apply bi.False_elim
+         | |- _ ⊢ True => apply bi.True_intro
+         (* | |- context[(_ ∧ ⌜_⌝)%I] => rewrite lprop_float *)
+         (* | |- ⌜?P⌝ ∧ ?Q ⊢ ?R => apply (land_prop_left (P := P) (Q := Q) (R := R)); intros ? *)
+         (* (* | |- !! ?P ⊢ _ => apply lprop_left; intros ? *) *)
+         | |- (∃ x : _, _) ⊢ _ => apply bi.exist_elim; intros ?
+         | |- _ ⊢ ∀ x : _, _ => apply bi.forall_intro; intros ?
+         (* | |- ?P ⊢ ?P ∨ _ => apply lor_right1; reflexivity *)
+         | |- ?P ∧ _  ⊢ ?P => apply bi.and_elim_l
+         | |- _  ∧ ?P ⊢ ?P => apply bi.and_elim_r
+         | |- ⌜_⌝ ∧ _ ⊢ _ => apply bi.impl_elim_r'
+         | |- _ ∧ ⌜_⌝ ⊢ _ => apply bi.impl_elim_l'
+         (* | H : ?P |- _ ⊢ ⌜?P⌝ => apply lprop_right; exact H *)
+         | |- _ ⊢ ⌜?x = ?x⌝ => apply bi.pure_intro; reflexivity
+         | |- _ ⊢ ⌜_⌝ → _ => rewrite bi.pure_impl_forall;
+                             apply bi.forall_intro; intros ?
+         (* | |- _ ⊢ ⌜_⌝ -∗ _ => apply lprop_intro_wand; intro *)
+         (* | H : _ \/ _ |- _ => destruct H *)
+         (* | |- _ ∨ _ ⊢ _ => apply lor_left *)
+         | |- _ ⊢ _ ∧ _ => apply bi.and_intro
+         (* (* Everything below is incomplete. *) *)
+         (* | |- _ ⊢ ∃ x : _, _ => eapply lex_right *)
+         (* | |- (∀ x : _, _) ⊢ _ => eapply lall_left *)
+         | |- _ ⊢ ⌜?P⌝  => is_ground P; apply bi.pure_intro; intuition auto; fail
+         | _ => easy
+         end).
+
+      Lemma wp_bind {A B} (m : CPureSpec A) (f : A -> CPureSpec B) (Φ : B -> L) :
+        bind m f Φ ⊣⊢ m (fun a => f a Φ).
+      Proof. easy. Qed.
+
+      Lemma wp_angelic_ctx {N : Set} {Δ : NCtx N Ty} (POST : NamedEnv Val Δ -> L) :
+        angelic_ctx Δ POST ⊣⊢ ∃ vs : NamedEnv Val Δ, POST vs.
+      Proof.
+        induction Δ; cbn; [|rewrite IHΔ]; solve_wp.
+        - iIntros "P". by iExists env.nil.
+        - iIntros "[%x P]". by iExists (env.snoc a _ x).
+        - iIntros "P". iExists E. by iExists v.
+      Qed.
+
+      Lemma wp_demonic_ctx {N : Set} {Δ : NCtx N Ty} (POST : NamedEnv Val Δ -> L) :
+        demonic_ctx Δ POST ⊣⊢ ∀ vs : NamedEnv Val Δ, POST vs.
+      Proof.
+        induction Δ; cbn; [|rewrite IHΔ]; solve_wp.
+        - iIntros "P". iApply "P".
+        - iIntros "P". iApply "P".
+        - iIntros "P %v". iApply "P".
+      Qed.
+
+      Lemma wp_angelic_list' {A} (xs : list A) (POST : A -> Prop) :
+        forall d,
+          angelic_list' d xs POST <->
+            exists x : A, List.In x (cons d xs) /\ POST x.
+      Proof.
+        induction xs; cbn; intros d.
+        - firstorder. now subst.
+        - firstorder. left. now subst.
+      Qed.
+
+      Lemma wp_angelic_list {A} (xs : list A) (POST : A -> Prop) :
+        angelic_list xs POST <->
+        exists x : A, List.In x xs /\ POST x.
+      Proof. destruct xs; cbn; [firstorder|apply wp_angelic_list']. Qed.
+
+    Lemma wp_demonic_list' {A} (xs : list A) (POST : A -> Prop) :
+      forall d,
+        demonic_list' d xs POST <->
+          forall x : A, List.In x (cons d xs) -> POST x.
+    Proof.
+      induction xs; cbn; intros d.
+      - firstorder. now subst.
+      - firstorder. now subst.
+    Qed.
+
+    Lemma wp_demonic_list {A} (xs : list A) (POST : A -> Prop) :
+      demonic_list xs POST <->
+      forall x : A, List.In x xs -> POST x.
+    Proof. destruct xs; cbn; [firstorder|apply wp_demonic_list']. Qed.
+
+    Lemma wp_angelic_pattern_match {N σ} (pat : Pattern (N:=N) σ) v
+      (Φ : MatchResult pat -> Prop) :
+      angelic_pattern_match pat v Φ <-> Φ (pattern_match_val pat v).
+    Proof.
+      unfold angelic_pattern_match, angelic_finite. cbn.
+      rewrite wp_angelic_list. setoid_rewrite wp_angelic_ctx.
+      split.
+      - intros (pc & Hin & δpc & <- & Hwp).
+        now rewrite pattern_match_val_inverse_right.
+      - set (mr := pattern_match_val pat v). intros HΦ.
+        exists (projT1 mr). split.
+        { rewrite <- base.elem_of_list_In. apply finite.elem_of_enum. }
+        exists (projT2 mr). split.
+        { subst mr. apply pattern_match_val_inverse_left. }
+        destruct mr. apply HΦ.
+    Qed.
+
+    Lemma wp_demonic_pattern_match {N σ} (pat : Pattern (N:=N) σ) v
+      (Φ : MatchResult pat -> Prop) :
+      demonic_pattern_match pat v Φ <-> Φ (pattern_match_val pat v).
+    Proof.
+      unfold demonic_pattern_match, demonic_finite. cbn.
+      rewrite wp_demonic_list. setoid_rewrite wp_demonic_ctx.
+      split.
+      - set (mr := pattern_match_val pat v). intros HΦ.
+        specialize (HΦ (projT1 mr)).
+        rewrite <- base.elem_of_list_In in HΦ.
+        specialize (HΦ (finite.elem_of_enum _) (projT2 mr)).
+        specialize (HΦ (pattern_match_val_inverse_left pat v)).
+        now destruct mr.
+      - intros HΦ pc Hin δpc <-. revert HΦ.
+        now rewrite pattern_match_val_inverse_right.
+    Qed.
+
+    Lemma wp_assert_eq_env {Δ : Ctx Ty} (δ δ' : Env Val Δ) :
+      forall Φ,
+        assert_eq_env δ δ' Φ <-> δ = δ' /\ Φ tt.
+    Proof.
+      induction δ; intros Φ; destruct (env.view δ'); cbn.
+      - intuition auto.
+      - rewrite IHδ, env.inversion_eq_snoc.
+        unfold assert_formula, assert_pathcondition.
+        intuition auto.
+    Qed.
+
+    Lemma wp_assert_eq_nenv {N} {Δ : NCtx N Ty} (δ δ' : NamedEnv Val Δ) :
+      forall Φ,
+        assert_eq_nenv δ δ' Φ <-> δ = δ' /\ Φ tt.
+    Proof.
+      induction δ; intros Φ; destruct (env.view δ'); cbn; unfold NamedEnv.
+      - intuition auto.
+      - rewrite IHδ, env.inversion_eq_snoc.
+        unfold assert_formula, assert_pathcondition.
+        intuition auto.
+    Qed.
+
+    (* For heap predicates and types of registers. *)
+    #[local] Set Equations With UIP.
+
+    Lemma wp_assert_eq_chunk (c c' : SCChunk) :
+      forall Φ,
+        assert_eq_chunk c c' Φ <-> c = c' /\ Φ tt.
+    Proof.
+      revert c'. induction c; intros c' Φ; destruct c'; cbn in *;
+        unfold error, FALSE; try (intuition discriminate).
+      - destruct eq_dec as [e|n]; cbn.
+        + rewrite wp_assert_eq_env. apply and_iff_compat_r'.
+          intros ?. destruct e; cbn. split; intros Heq.
+          * now f_equal.
+          * now dependent elimination Heq.
+        + split; try contradiction. intros [Heq Hwp]. apply n.
+          now dependent elimination Heq.
+      - destruct eq_dec_het as [e|n]; cbn.
+        + apply and_iff_compat_r'. intros ?.
+          dependent elimination e; cbn.
+          split; intros Heq.
+          * now f_equal.
+          * now dependent elimination Heq.
+        + split; try contradiction. intros [Heq Hwp]. apply n.
+          now dependent elimination Heq.
+      - rewrite IHc1, IHc2. intuition congruence.
+      - rewrite IHc1, IHc2. intuition congruence.
+    Qed.
+
+    Lemma replay_sound {Σ} (s : 𝕊 Σ) (ι : Valuation Σ) :
+      replay s ι -> SymProp.safe s ι.
+    Proof.
+      unfold replay, run.
+      induction s; cbn.
+      - intros [|]; intuition auto.
+      - intros []; intuition auto.
+      - inversion 1.
+      - auto.
+      - intros []. intuition auto.
+      - intuition auto.
+      - apply ex_impl_morphism. intros v; red; apply IHs.
+      - apply all_impl_morphism. intros v; red; apply IHs.
+      - intros []. intuition auto.
+      - intuition auto.
+      - inversion 1.
+      - inversion 1.
+      - unfold debug. apply IHs.
+    Qed.
+
+    Section WithBI.
+
+      Import iris.bi.interface iris.bi.derived_laws iris.bi.extensions.
+
+      Context {L} {biA : BiAffine L} {PI : PredicateDef L}.
+
+      Lemma wp_consume_chunk (c : SCChunk) (h : SCHeap) (Φ : SCHeap -> Prop) :
+        consume_chunk c h Φ ->
+        (interpret_scheap h ⊢
+         interpret_scchunk c ∗ ∃ h', interpret_scheap h' ∧ ⌜Φ h'⌝).
+      Proof.
+        unfold consume_chunk. cbn.
+        rewrite wp_angelic_list.
+        intros ([c' h'] & HIn & H). cbn in H.
+        rewrite CPureSpec.wp_assert_eq_chunk in H.
+        destruct H as [Heq Hput]. subst. hnf in Hput.
+        apply in_heap_extractions in HIn. rewrite HIn.
+        apply bi.sep_mono'; [easy|].
+        apply bi.exist_intro' with h'.
+        apply bi.and_intro; auto.
+      Qed.
+      #[global] Arguments consume_chunk : simpl never.
+
+      Lemma wp_produce_chunk (c : SCChunk) (h : SCHeap) (Φ : SCHeap -> Prop) :
+        produce_chunk c h Φ ->
+        (interpret_scheap h ⊢
+         interpret_scchunk c -∗ ∃ h', interpret_scheap h' ∧ ⌜Φ h'⌝).
+      Proof.
+        cbn. intros HΦ. apply bi.wand_intro_l.
+        apply bi.exist_intro' with (c :: h).
+        apply bi.and_intro; auto.
+      Qed.
+      #[global] Arguments produce_chunk : simpl never.
+
+      Lemma wp_read_register {τ} (reg : 𝑹𝑬𝑮 τ) (h0 : SCHeap) Φ :
+        read_register reg h0 Φ ->
+        interpret_scheap h0 ⊢
+        ∃ v, lptsreg reg v ∗
+             (lptsreg reg v -∗ ∃ h1, interpret_scheap h1 ∧ ⌜Φ (v, h1)⌝).
+      Proof.
+        cbv [read_register angelic pure bind].
+        intros [v ->%wp_consume_chunk].
+        apply bi.exist_intro' with v.
+        apply bi.sep_mono'. easy.
+        apply bi.exist_elim. intros h1.
+        apply bi.pure_elim_r.
+        intros ->%wp_produce_chunk.
+        now apply bi.wand_mono'.
+      Qed.
+
+      Lemma wp_write_register {τ} (reg : 𝑹𝑬𝑮 τ) (vnew : Val τ) (h0 : SCHeap) Φ :
+        write_register reg vnew h0 Φ ->
+        interpret_scheap h0 ⊢
+        ∃ vold, lptsreg reg vold ∗
+                (lptsreg reg vnew -∗ ∃ h1, interpret_scheap h1 ∧ ⌜Φ (vnew, h1)⌝).
+      Proof.
+        cbv [write_register angelic pure bind].
+        intros [v ->%wp_consume_chunk].
+        apply bi.exist_intro' with v.
+        apply bi.sep_mono'. easy.
+        apply bi.exist_elim. intros h1.
+        apply bi.pure_elim_r.
+        intros ->%wp_produce_chunk.
+        now apply bi.wand_mono'.
+      Qed.
+
+    End WithBI.
+
+  End CPureSpec.
+  Export (hints) CPureSpec.
+
+  Definition CHeapSpec (A : Type) : Type :=
+    (A -> SCHeap -> Prop) -> SCHeap -> Prop.
+
+  Definition MHeapSpec [A] (MA : relation A) : relation (CHeapSpec A) :=
+    (MA ==> SCHeap ::> impl) ==> SCHeap ::> impl.
+
+  Module CHeapSpec.
+
+    Definition run : CHeapSpec unit -> Prop :=
+      (* We use the FINISH alias of True for the purpose
+         of counting nodes in a shallowly-generated VC. *)
+      fun m => m (fun _ h1 => FINISH) List.nil.
+
+    Definition lift_purespec {A : Type} :
+      CPureSpec A -> CHeapSpec A :=
+      fun m Φ h0 => m (fun a1 => Φ a1 h0).
+
+    Definition pure {A} a := lift_purespec (@CPureSpec.pure A a).
+
+    Definition bind {A B} : CHeapSpec A -> (A -> CHeapSpec B) -> CHeapSpec B :=
+      fun m f Φ h => m (fun a1 => f a1 Φ) h.
+
+    Module Import notations.
+      Notation "' x <- ma ;; mb" :=
+        (bind ma (fun x => mb))
+          (at level 80, x pattern, ma at next level, mb at level 200, right associativity,
+             format "' x  <-  ma  ;;  mb").
+      Notation "x <- ma ;; mb" :=
+        (bind ma (fun x => mb))
+          (at level 80, ma at level 90, mb at level 200, right associativity).
+      Notation "ma ;; mb" := (bind ma (fun _ => mb)).
+    End notations.
+
+    Definition error {A} : CHeapSpec A :=
+      fun _ _ => FALSE.
+
+    Definition debug {A} : CHeapSpec A -> CHeapSpec A :=
+      fun m => m.
+
+    Definition angelic_binary {A} : CHeapSpec A -> CHeapSpec A -> CHeapSpec A :=
+      fun m1 m2 Φ h => m1 Φ h \/ m2 Φ h.
+    Definition demonic_binary {A} : CHeapSpec A -> CHeapSpec A -> CHeapSpec A :=
+      fun m1 m2 Φ h => m1 Φ h /\ m2 Φ h.
+
+    Definition angelic (σ : Ty) : CHeapSpec (Val σ) :=
+      lift_purespec (CPureSpec.angelic σ).
+    #[global] Arguments angelic σ Φ : rename.
+    Definition demonic (σ : Ty) : CHeapSpec (Val σ) :=
+      lift_purespec (CPureSpec.demonic σ).
+    #[global] Arguments demonic σ Φ : rename.
+
+    Definition angelic_ctx {N} (Δ : NCtx N Ty) : CHeapSpec (NamedEnv Val Δ) :=
+      lift_purespec (CPureSpec.angelic_ctx Δ).
+    #[global] Arguments angelic_ctx {N} Δ.
+    Definition demonic_ctx {N} (Δ : NCtx N Ty) : CHeapSpec (NamedEnv Val Δ) :=
+      lift_purespec (CPureSpec.demonic_ctx Δ).
+    #[global] Arguments demonic_ctx {N} Δ.
+
+    Definition assert_formula : Prop -> CHeapSpec unit :=
+      fun fml => lift_purespec (CPureSpec.assert_formula fml).
+    Definition assume_formula : Prop -> CHeapSpec unit :=
+      fun fml => lift_purespec (CPureSpec.assume_formula fml).
+
+    Definition produce_chunk (c : SCChunk) : CHeapSpec unit :=
+      fun Φ h => CPureSpec.produce_chunk c h (Φ tt).
+    Definition consume_chunk (c : SCChunk) : CHeapSpec unit :=
+      fun Φ h => CPureSpec.consume_chunk c h (Φ tt).
+
+    Definition read_register {τ} (reg : 𝑹𝑬𝑮 τ) : CHeapSpec (Val τ) :=
+      fun Φ h => CPureSpec.read_register reg h (fun '(t,h') => Φ t h').
+    Definition write_register {τ} (reg : 𝑹𝑬𝑮 τ) (v : Val τ) : CHeapSpec (Val τ) :=
+      fun Φ h => CPureSpec.write_register reg v h (fun '(v',h') => Φ v' h').
+
+    Fixpoint produce {Σ} (asn : Assertion Σ) (ι : Valuation Σ) : CHeapSpec unit :=
+      match asn with
+      | asn.formula fml =>
+          assume_formula (instprop fml ι)
+      | asn.chunk c =>
+          produce_chunk (inst c ι)
+      | asn.chunk_angelic c =>
+          produce_chunk (inst c ι)
+      | asn.pattern_match s pat rhs =>
+          '(existT pc δpc) <-
+            lift_purespec (CPureSpec.demonic_pattern_match pat (inst s ι)) ;;
+          produce (rhs pc) (ι ►► δpc)
+      | asn.sep a1 a2 =>
+          _ <- produce a1 ι ;;
+          produce a2 ι
+      | asn.or a1 a2 =>
+          demonic_binary (produce a1 ι) (produce a2 ι)
+      | asn.exist ς τ a =>
+          t <- demonic τ ;;
+          produce a (env.snoc ι (ς∷τ) t)
+      | asn.debug =>
+          debug (pure tt)
+      end.
+
+    Fixpoint consume {Σ} (asn : Assertion Σ) (ι : Valuation Σ) : CHeapSpec unit :=
+      match asn with
+      | asn.formula fml =>
+          assert_formula (instprop fml ι)
+      | asn.chunk c =>
+          consume_chunk (inst c ι)
+      | asn.chunk_angelic c =>
+          consume_chunk (inst c ι)
+      | asn.pattern_match s pat rhs =>
+          '(existT pc δpc) <-
+            lift_purespec (CPureSpec.angelic_pattern_match pat (inst s ι)) ;;
+          consume (rhs pc) (ι ►► δpc)
+      | asn.sep a1 a2 =>
+          _ <- consume a1 ι ;;
+          consume a2 ι
+      | asn.or a1 a2 =>
+          angelic_binary (consume a1 ι) (consume a2 ι)
+      | asn.exist ς τ a =>
+          t <- angelic τ ;;
+          consume a (env.snoc ι (ς∷τ) t)
+      | asn.debug =>
+          debug (pure tt)
+      end.
+
+    Definition call_contract [Δ τ] (c : SepContract Δ τ) (args : CStore Δ) : CHeapSpec (Val τ) :=
+      match c with
+      | MkSepContract _ _ Σe δ req result ens =>
+          ι <- lift_purespec (CPureSpec.angelic_ctx Σe) ;;
+          lift_purespec (CPureSpec.assert_eq_nenv (inst δ ι) args) ;;
+          consume req ι ;;
+          v <- demonic τ ;;
+          produce ens (env.snoc ι (result∷τ) v) ;;
+          pure v
+      end.
+
+    Definition call_lemma [Δ] (lem : Lemma Δ) (vs : CStore Δ) : CHeapSpec unit :=
+      match lem with
+      | MkLemma _ Σe δ req ens =>
+          ι <- lift_purespec (CPureSpec.angelic_ctx Σe) ;;
+          lift_purespec (CPureSpec.assert_eq_nenv (inst δ ι) vs) ;;
+          consume req ι ;;
+          produce ens ι
+      end.
+
+    #[export] Instance mon_run :
+      Monotonic (MHeapSpec eq ==> impl) run.
+    Proof. intros m1 m2 mm. now apply mm. Qed.
+
+    Lemma mon_lift_purespec' `{MA : relation A} :
+      Monotonic (MPureSpec MA ==> MHeapSpec MA) (lift_purespec).
+    Proof. intros ? ? rm ? ? rΦ h. apply rm. intros ? ? ra. now apply rΦ. Qed.
+
+    #[export] Instance mon_lift_purespec `{MA : relation A} m :
+      Monotonic (MPureSpec MA) m -> Monotonic (MHeapSpec MA) (lift_purespec m).
+    Proof. intros rm. now apply mon_lift_purespec'. Qed.
+
+    Lemma mon_pure' `{MA : relation A} :
+      Monotonic (MA ==> MHeapSpec MA) pure.
+    Proof. firstorder. Qed.
+
+    #[export] Instance mon_pure `{MA : relation A} x :
+      Monotonic MA x -> Monotonic (MHeapSpec MA) (pure x).
+    Proof. firstorder. Qed.
+
+    Lemma mon_bind' `{MA : relation A, RB : relation B} :
+      Monotonic (MHeapSpec MA ==> (MA ==> MHeapSpec RB) ==> MHeapSpec RB) bind.
+    Proof.
+      intros ? ? rm ? ? rf ? ? rΦ. apply rm. intros ? ? ra.
+      apply rf. apply ra. intros ? ? rb. apply rΦ, rb.
+    Qed.
+
+    #[export] Instance mon_bind `{MA : relation A, RB : relation B}
+      (m : CHeapSpec A) (f : A -> CHeapSpec B) :
+      Monotonic (MHeapSpec MA) m ->
+      Monotonic (MA ==> MHeapSpec RB) f ->
+      Monotonic (MHeapSpec RB) (bind m f).
+    Proof. intros rm rf. eapply mon_bind'; eauto. Qed.
+
+    #[export] Instance mon_error `{MA : relation A} :
+      Monotonic (MHeapSpec MA) error.
+    Proof. now unfold error. Qed.
+
+    #[export] Instance mon_debug `{MA : relation A} m :
+      Monotonic (MHeapSpec MA) m -> Monotonic (MHeapSpec MA) (debug m).
+    Proof. now unfold debug. Qed.
+
+    #[export] Instance mon_angelic_binary `{MA : relation A} m1 m2 :
+      Monotonic (MHeapSpec MA) m1 -> Monotonic (MHeapSpec MA) m2 ->
+      Monotonic (MHeapSpec MA) (angelic_binary m1 m2).
+    Proof. firstorder. Qed.
+
+    #[export] Instance mon_demonic_binary `{MA : relation A} m1 m2 :
+      Monotonic (MHeapSpec MA) m1 -> Monotonic (MHeapSpec MA) m2 ->
+      Monotonic (MHeapSpec MA) (demonic_binary m1 m2).
+    Proof. firstorder. Qed.
+
+    #[global] Typeclasses Opaque run lift_purespec pure bind debug angelic_binary
+      demonic_binary.
+
+    #[export] Instance mon_angelic σ :
+      Monotonic (MHeapSpec eq) (angelic σ).
+    Proof. typeclasses eauto. Qed.
+    #[export] Instance mon_demonic σ :
+      Monotonic (MHeapSpec eq) (demonic σ).
+    Proof. typeclasses eauto. Qed.
+
+    #[export] Instance mon_assert_formula fml :
+      Monotonic (MHeapSpec eq) (assert_formula fml).
+    Proof. firstorder. Qed.
+    #[export] Instance mon_assume_formula fml :
+      Monotonic (MHeapSpec eq) (assume_formula fml).
+    Proof. firstorder. Qed.
+
+    #[export] Instance mon_produce_chunk c : Monotonic (MHeapSpec eq) (produce_chunk c).
+    Proof.
+      intros Φ1 Φ2 mΦ h.
+      apply CPureSpec.mon_produce_chunk.
+      intros ? ? ->. now apply mΦ.
+    Qed.
+
+    #[export] Instance mon_consume_chunk c : Monotonic (MHeapSpec eq) (consume_chunk c).
+    Proof.
+      intros Φ1 Φ2 mΦ h.
+      apply CPureSpec.mon_consume_chunk.
+      intros ? ? ->. now apply mΦ.
+    Qed.
+
+    #[export] Instance mon_read_register {τ} (reg : 𝑹𝑬𝑮 τ) :
+      Monotonic (MHeapSpec eq) (read_register reg).
+    Proof.
+      intros Φ1 Φ2 mΦ h.
+      apply CPureSpec.mon_read_register.
+      intros ? [] ->. now apply mΦ.
+    Qed.
+
+    #[export] Instance mon_write_register {τ} (reg : 𝑹𝑬𝑮 τ) (v : Val τ) :
+      Monotonic (MHeapSpec eq) (write_register reg v).
+    Proof.
+      intros Φ1 Φ2 mΦ h.
+      apply CPureSpec.mon_write_register.
+      intros ? [] ->. now apply mΦ.
+    Qed.
+
+    #[global] Typeclasses Opaque angelic demonic assert_formula assume_formula
+      produce_chunk consume_chunk read_register write_register.
+
+    #[export] Instance mon_produce {Σ} (asn : Assertion Σ) ι :
+      Monotonic (MHeapSpec eq) (produce asn ι).
+    Proof. induction asn; cbn; typeclasses eauto. Qed.
+
+    #[export] Instance mon_consume {Σ} (asn : Assertion Σ) ι :
+      Monotonic (MHeapSpec eq) (consume asn ι).
+    Proof. induction asn; cbn; typeclasses eauto. Qed.
+
+    #[export] Instance mon_call_contract
+      [Δ τ] (c : SepContract Δ τ) (args : CStore Δ) :
+      Monotonic (MHeapSpec eq) (call_contract c args).
+    Proof. destruct c; typeclasses eauto. Qed.
+
+    #[export] Instance mon_call_lemma
+      [Δ] (lem : Lemma Δ) (vs : CStore Δ) :
+      Monotonic (MHeapSpec eq) (call_lemma lem vs).
+    Proof. destruct lem; typeclasses eauto. Qed.
+
+    #[global] Typeclasses Opaque produce consume call_contract call_lemma.
+
+    Section WithBI.
+
+      Import iris.proofmode.tactics.
+
+      Context {L} {biA : BiAffine L} {PI : PredicateDef L}.
+
+      #[local] Arguments CHeapSpec.bind {_ _} _ _ _ /.
+      #[local] Arguments CHeapSpec.angelic_binary {_} _ _ /.
+      #[local] Arguments CHeapSpec.demonic_binary {_} _ _ /.
+      #[local] Arguments CHeapSpec.lift_purespec {_} _ _ /.
+
+      Lemma consume_sound {Σ} {ι : Valuation Σ} {asn : Assertion Σ} :
+        forall (Φ : unit -> SCHeap -> Prop) h,
+          consume asn ι Φ h ->
+          (interpret_scheap h ⊢ asn.interpret asn ι ∗ ∃ h', interpret_scheap h' ∧ ⌜ Φ tt h' ⌝)%I.
+      Proof.
+        induction asn; cbn - [inst inst_term]; intros Φ h1.
+        - intros [Hfmle HΦ]. rewrite <-bi.emp_sep at 1. apply bi.sep_mono'.
+          + rewrite bi.and_emp; auto.
+          + apply bi.exist_intro' with h1. apply bi.and_intro; auto.
+        - intros ->%CPureSpec.wp_consume_chunk. now rewrite interpret_scchunk_inst.
+        - intros ->%CPureSpec.wp_consume_chunk. now rewrite interpret_scchunk_inst.
+        - rewrite CPureSpec.wp_angelic_pattern_match.
+          destruct pattern_match_val; auto.
+        - intros ->%IHasn1. rewrite -bi.sep_assoc. apply bi.sep_mono'; [easy|].
+          apply bi.exist_elim. intros h2. apply bi.pure_elim_r. apply IHasn2.
+        - intros [->%IHasn1 | ->%IHasn2]; apply bi.sep_mono'; auto.
+        - intros (v & ->%IHasn). apply bi.sep_mono'; [|easy].
+          now apply bi.exist_intro' with v.
+        - intros HΦ. rewrite bi.emp_sep. apply bi.exist_intro' with h1.
+          apply bi.and_intro; auto.
+      Qed.
+
+      Lemma produce_sound {Σ} {ι : Valuation Σ} {asn : Assertion Σ} :
+        forall (Φ : unit -> SCHeap -> Prop) h,
+          produce asn ι Φ h ->
+          (interpret_scheap h ⊢
+             asn.interpret asn ι -∗ ∃ h', interpret_scheap h' ∧ ⌜Φ tt h'⌝).
+      Proof.
+        induction asn; cbn - [CPureSpec.assume_formula inst inst_term]; intros Φ h.
+        - iIntros (HΦ) "Hh [%Hfml _]". iExists h. auto.
+        - intros ->%CPureSpec.wp_produce_chunk; now rewrite interpret_scchunk_inst.
+        - intros ->%CPureSpec.wp_produce_chunk; now rewrite interpret_scchunk_inst.
+        - rewrite CPureSpec.wp_demonic_pattern_match.
+          destruct pattern_match_val; auto.
+        - iIntros (Hprod1) "H [Hasn1 Hasn2]".
+          iPoseProof (IHasn1 _ _ _ Hprod1 with "H Hasn1") as "(%h2 & H & %Hprod2)".
+          iPoseProof (IHasn2 _ _ _ Hprod2 with "H Hasn2") as "(%h3 & H & %HΦ)".
+          iExists h3. auto.
+        - iIntros ([HΦ1 HΦ2]) "Hh [Hasn1|Hasn2]".
+          iApply (IHasn1 with "Hh Hasn1"); auto.
+          iApply (IHasn2 with "Hh Hasn2"); auto.
+        - iIntros (HΦ) "Hh [%v Hasn]".
+          now iApply (IHasn with "Hh Hasn").
+        - iIntros (HΦ) "Hh _". iExists h. auto.
+      Qed.
+
+    End WithBI.
+
+  End CHeapSpec.
+  Export (hints) CHeapSpec.
+
+  Module CStatistics.
+
+    Inductive PropShape : Type :=
+    | psfork (P Q : PropShape)
+    | psquant (P : PropShape)
+    | pspruned
+    | psfinish
+    | psother.
+
+    Fixpoint shape_to_stats (s : PropShape) : Stats :=
+      match s with
+      | psfork p q => plus_stats (shape_to_stats p) (shape_to_stats q)
+      | psquant p  => shape_to_stats p
+      | pspruned   => {| branches := 1; pruned := 1 |}
+      | psfinish   => {| branches := 1; pruned := 0 |}
+      | psother     => {| branches := 0; pruned := 0 |}
+      end.
+
+    (* See: Building a Reification Tactic that Recurses Under Binders *)
+    (*          http://adam.chlipala.net/cpdt/html/Cpdt.Reflection.html *)
+
+    (*          This calculates a deeply-embedded PropShape for a given Prop P *)
+    (*          for which we can then run shape_to_stats to calculate the *)
+    (*          number of different kinds of execution paths. *)
+    Ltac reifyProp P :=
+      match eval simpl in P with
+      | forall (x : ?T), TRUE => pspruned
+      | forall (x : ?T), FALSE => pspruned
+      | forall (x : ?T), FINISH => psfinish
+      | forall (x : ?T), True => psother
+      | forall (x : ?T), False => psother
+      | forall (x : ?T), @?P1 x /\ @?P2 x =>
+          let t1 := reifyProp (forall x : T, P1 x) in
+          let t2 := reifyProp (forall x : T, P2 x) in
+          constr:(psfork t1 t2)
+      | forall (x : ?T), @?P1 x \/ @?P2 x =>
+          let t1 := reifyProp (forall x : T, P1 x) in
+          let t2 := reifyProp (forall x : T, P2 x) in
+          constr:(psfork t1 t2)
+      | forall (x : ?T), @?P1 x -> @?P2 x =>
+          let t1 := reifyProp (forall x : T, P1 x) in
+          let t2 := reifyProp (forall x : T, P2 x) in
+          constr:(psfork t1 t2)
+      | forall (x : ?T), forall (v : ?U), @?P x v =>
+          let t := reifyProp (forall xv : T * U, P (fst xv) (snd xv)) in
+          constr:(psquant t)
+      | forall (x : ?T), exists (v : ?U), @?P x v =>
+          let t := reifyProp (forall xv : T * U, P (fst xv) (snd xv)) in
+          constr:(psquant t)
+      | forall (x : ?T), _ = _ => psother
+      | forall (x : ?T), Z.le _ _ => psother
+      (* | _ => constr:(sprop P) *)
+      end.
+
+    (* This typeclass approach seems to be much faster than the reifyProp *)
+    (* tactic above. *)
+    Class ShallowStats (P : Prop) :=
+      stats : Stats.
+    Arguments stats P {_}.
+
+    (* We make these instances global so that users can simply use the *)
+    (* calc tactic qualified without importing the rest of this module. *)
+    #[global] Instance stats_true : ShallowStats TRUE :=
+      {| branches := 1; pruned := 1 |}.
+    #[global] Instance stats_false : ShallowStats FALSE :=
+      {| branches := 1; pruned := 1 |}.
+    #[global] Instance stats_finish : ShallowStats FINISH :=
+      {| branches := 1; pruned := 0 |}.
+    (* We do not count regular True and False towards the statistics *)
+    (* because they do not (should not) represent leaves of the shallow *)
+    (* execution. *)
+    #[global] Instance stats_true' : ShallowStats True :=
+      {| branches := 0; pruned := 0 |}.
+    #[global] Instance stats_false' : ShallowStats False :=
+      {| branches := 0; pruned := 0 |}.
+
+    #[global] Instance stats_eq {A} {x y : A} : ShallowStats (x = y) :=
+      {| branches := 0; pruned := 0 |}.
+    #[global] Instance stats_zle {x y : Z} : ShallowStats (Z.le x y) :=
+      {| branches := 0; pruned := 0 |}.
+
+    #[global] Instance stats_and `{ShallowStats P, ShallowStats Q} :
+      ShallowStats (P /\ Q) := plus_stats (stats P) (stats Q).
+    #[global] Instance stats_or `{ShallowStats P, ShallowStats Q} :
+      ShallowStats (P \/ Q) := plus_stats (stats P) (stats Q).
+    #[global] Instance stats_impl `{ShallowStats P, ShallowStats Q} :
+      ShallowStats (P -> Q) := plus_stats (stats P) (stats Q).
+
+    Section WithUndefined.
+
+      Variable undefined : forall A, A.
+
+      #[global] Instance stats_forall {A} {B : A -> Prop} {SP : forall a, ShallowStats (B a)} :
+        ShallowStats (forall a : A, B a) := SP (undefined A).
+      #[global] Instance stats_exists {A} {B : A -> Prop} {SP : forall a, ShallowStats (B a)} :
+        ShallowStats (exists a : A, B a) := SP (undefined A).
+
+    End WithUndefined.
+
+  End CStatistics.
+
+End ShallowMonadsOn.
